@prefix : <http://w3id.org/CEON/ontology/processODP/> .
@prefix odp: <http://www.ontologydesignpatterns.org/schemas/cpannotationschema.owl#> .
@prefix owl: <http://www.w3.org/2002/07/owl#> .
@prefix rdf: <http://www.w3.org/1999/02/22-rdf-syntax-ns#> .
@prefix xml: <http://www.w3.org/XML/1998/namespace> .
@prefix xsd: <http://www.w3.org/2001/XMLSchema#> .
@prefix rdfs: <http://www.w3.org/2000/01/rdf-schema#> .
@prefix vann: <http://purl.org/vocab/vann/> .
@prefix dcterms: <http://purl.org/dc/terms/> .
@prefix resourceODP: <http://w3id.org/CEON/ontology/resourceODP/> .
@base <http://w3id.org/CEON/ontology/processODP/> .

<http://w3id.org/CEON/ontology/processODP/> rdf:type owl:Ontology ;
                                             owl:versionIRI <http://w3id.org/CEON/ontology/processODP/0.5/> ;
                                             dcterms:contributor "Eva Blomqvist" ,
                                                                 "Mikael Lindecrantz" ,
                                                                 "Robin Keskisärkkä" ;
                                             dcterms:created "2025-05-20"^^xsd:date ;
                                             dcterms:issued "2025-06-30"^^xsd:date ;
                                             dcterms:publisher "Onto-DESIDE" ;
                                             dcterms:creator "Huanyu Li" ;
                                             dcterms:description "A core ODP of the CEON ontology network, defining aspects of the process concept." ;
                                             dcterms:license "https://creativecommons.org/licenses/by/4.0/" ;
                                             dcterms:title "Circular Economy Ontology Network (CEON) - Process ODP" ;
                                             vann:preferredNamespacePrefix "ceon-processODP" ;
                                             vann:preferredNamespaceUri "http://w3id.org/CEON/ontology/processODP/" ;
                                             odp:coversRequirements "Covers the following requirements from Onto-DESIDE D3.1: CVN-Process-3,4,5, C3-1, C4-2, C4-5, C4-7, C4-9, C13-2, E2-6" ,
                                                                    "Covers the following requirements from Onto-DESIDE D3.2: CE1-1, CE3-5, CE7-4, CE7-5, CE8-2, CE10-7, CE12-1, C3-1, C4-2, C4-5, C4-7, C4-9, C13-2, E2-6" ;
                                             rdfs:comment "A core ODP of the CEON ontology network, defining aspects of the process concept." ;
                                             rdfs:seeAlso <https://github.com/LiUSemWeb/CEON> ;
                                             owl:priorVersion 0.4 ;
                                             owl:versionInfo 0.5 .

#################################################################
#    Annotation properties
#################################################################

###  http://purl.org/dc/terms/contributor
#dcterms:contributor rdf:type owl:AnnotationProperty .



#################################################################
#    Object Properties
#################################################################

###  http://w3id.org/CEON/ontology/processODP/duringTime
:duringTime rdf:type owl:ObjectProperty ;
            rdfs:range :TimeInterval ;
            rdfs:comment "The time interval during which something, e.g. a process or event, takes place." ;
            rdfs:label "during time" .


###  http://w3id.org/CEON/ontology/processODP/hasInput
:hasInput rdf:type owl:ObjectProperty ;
          rdfs:domain :Process ;
          rdfs:comment "The inputs to a process or event." ;
          rdfs:label "has input" .


###  http://w3id.org/CEON/ontology/processODP/hasOutput
:hasOutput rdf:type owl:ObjectProperty ;
           rdfs:domain :Process ;
           rdfs:comment "The output of a process or event." ;
           rdfs:label "has output" .


###  http://w3id.org/CEON/ontology/processODP/hasPart
:hasPart rdf:type owl:ObjectProperty ,
                  owl:TransitiveProperty ;
         rdfs:comment "A process or event can consist of several parts, which are sub-processes (e.g. steps) or events." ;
         rdfs:label "has part" .


###  http://w3id.org/CEON/ontology/processODP/isSettingFor
:isSettingFor rdf:type owl:ObjectProperty ;
              rdfs:domain :Situation ;
              rdfs:comment "The thing(s) that this situation is the setting for, e.g. a resource that is in a certain state." ;
              rdfs:label "is the setting for" .


###  http://w3id.org/CEON/ontology/processODP/occursAtLocation
:occursAtLocation rdf:type owl:ObjectProperty ;
                  rdfs:subPropertyOf :isSettingFor ;
                  rdfs:range <http://w3id.org/CEON/ontology/location/Location> ;
                  rdfs:comment "The location in which something (e.g. an event or process) takes place, e.g. the factory location where something is manufactured." ;
                  rdfs:label "occurs at location" .


#################################################################
#    Data properties
#################################################################

###  http://w3id.org/CEON/ontology/processODP/endTime
:endTime rdf:type owl:DatatypeProperty ;
         rdfs:domain :TimeInterval ;
         rdfs:range xsd:dateTime ;
         rdfs:comment "Represents the end time of a time interval." ;
         rdfs:label "end time" .


###  http://w3id.org/CEON/ontology/processODP/startTime
:startTime rdf:type owl:DatatypeProperty ;
           rdfs:domain :TimeInterval ;
           rdfs:range xsd:dateTime ;
           rdfs:comment "Represents the start time of a time interval." ;
           rdfs:label "start time" .


#################################################################
#    Classes
#################################################################

###  http://w3id.org/CEON/ontology/location/Location
<http://w3id.org/CEON/ontology/location/Location> rdf:type owl:Class .


###  http://w3id.org/CEON/ontology/processODP/Event
:Event rdf:type owl:Class ;
       rdfs:comment "Something that happens within a given context or (short) timeframe." ;
       rdfs:label "Event".


###  http://w3id.org/CEON/ontology/processODP/Process
:Process rdf:type owl:Class ;
         rdfs:comment "Something that takes place over a (longer) period of time and changes some state of affairs."@en ;
         rdfs:label "Process" .


###  http://w3id.org/CEON/ontology/processODP/Situation
:Situation rdf:type owl:Class ;
           rdfs:subClassOf [ rdf:type owl:Restriction ;
                             owl:onProperty :isSettingFor ;
                             owl:someValuesFrom owl:Thing
                           ] ;
           rdfs:comment "A situation that may involve some resources and actors, i.e. a state of affairs at a certain point in time." ;
           rdfs:label "Situation" .


###  http://w3id.org/CEON/ontology/processODP/TimeInterval
:TimeInterval rdf:type owl:Class ;
              rdfs:comment "A temporal entity has a starting time and an ending time." ;
              rdfs:label "Time Interval" .


###  Generated by the OWL API (version 4.5.29.2024-05-13T12:11:03Z) https://github.com/owlcs/owlapi
