<?xml version="1.0" encoding="utf-8"?>
<rdf:RDF
   xmlns:dcterms="http://purl.org/dc/terms/"
   xmlns:odp="http://www.ontologydesignpatterns.org/schemas/cpannotationschema.owl#"
   xmlns:owl="http://www.w3.org/2002/07/owl#"
   xmlns:rdf="http://www.w3.org/1999/02/22-rdf-syntax-ns#"
   xmlns:rdfs="http://www.w3.org/2000/01/rdf-schema#"
   xmlns:vann="http://purl.org/vocab/vann/"
>
  <rdf:Description rdf:about="http://w3id.org/CEON/ontology/material/Lanthanum">
    <rdf:type rdf:resource="http://www.w3.org/2002/07/owl#Class"/>
    <rdfs:subClassOf rdf:resource="http://w3id.org/CEON/ontology/material/RareEarthElement"/>
    <rdfs:comment>Lanthanum is a chemical element with the symbol Lal and atomic number 57.</rdfs:comment>
    <rdfs:label>Lanthanum</rdfs:label>
  </rdf:Description>
  <rdf:Description rdf:about="http://w3id.org/CEON/ontology/material/Magnesium">
    <rdf:type rdf:resource="http://www.w3.org/2002/07/owl#Class"/>
    <rdfs:subClassOf rdf:resource="http://w3id.org/CEON/ontology/material/ChemicalElement"/>
    <rdfs:comment>Magnesium is a chemical element with the symbol Mg and atomic number 12.</rdfs:comment>
    <rdfs:label>Magnesium</rdfs:label>
  </rdf:Description>
  <rdf:Description rdf:about="http://w3id.org/CEON/ontology/material/Cerium">
    <rdf:type rdf:resource="http://www.w3.org/2002/07/owl#Class"/>
    <rdfs:subClassOf rdf:resource="http://w3id.org/CEON/ontology/material/RareEarthElement"/>
    <rdfs:comment>Cerium is a chemical element with the symbol Ce and atomic number 58.</rdfs:comment>
    <rdfs:label>Cerium</rdfs:label>
  </rdf:Description>
  <rdf:Description rdf:about="http://w3id.org/CEON/ontology/material/Dysprosium">
    <rdf:type rdf:resource="http://www.w3.org/2002/07/owl#Class"/>
    <rdfs:subClassOf rdf:resource="http://w3id.org/CEON/ontology/material/RareEarthElement"/>
    <rdfs:comment>Dysprosium is a chemical element with the symbol Dy and atomic number 66.</rdfs:comment>
    <rdfs:label>Dysorisium</rdfs:label>
  </rdf:Description>
  <rdf:Description rdf:about="http://w3id.org/CEON/ontology/material/Ytterbium">
    <rdf:type rdf:resource="http://www.w3.org/2002/07/owl#Class"/>
    <rdfs:subClassOf rdf:resource="http://w3id.org/CEON/ontology/material/RareEarthElement"/>
    <rdfs:comment>Yteerbium is a chemical element with the symbol Yb and atomic number 70.</rdfs:comment>
    <rdfs:label>Ytterbium</rdfs:label>
  </rdf:Description>
  <rdf:Description rdf:about="http://w3id.org/CEON/ontology/material/Aluminum">
    <rdf:type rdf:resource="http://www.w3.org/2002/07/owl#Class"/>
    <rdfs:subClassOf rdf:resource="http://w3id.org/CEON/ontology/material/ChemicalElement"/>
    <rdfs:comment>Aluminum is a chemical element with the symbol Al and atomic number 13.</rdfs:comment>
    <rdfs:label>Aluminum</rdfs:label>
  </rdf:Description>
  <rdf:Description rdf:about="http://w3id.org/CEON/ontology/material/ChemicalSubstance">
    <rdf:type rdf:resource="http://www.w3.org/2002/07/owl#Class"/>
    <rdfs:subClassOf rdf:resource="http://w3id.org/CEON/ontology/material/ChemicalEntity"/>
    <rdfs:comment>A chemical substance is made up of a collection of molecular entities.</rdfs:comment>
    <rdfs:label>Chemical Substance</rdfs:label>
    <rdfs:seeAlso>http://emmo.info/emmo#EMMO_df96cbb6_b5ee_4222_8eab_b3675df24bea</rdfs:seeAlso>
    <rdfs:seeAlso>http://purl.obolibrary.org/obo/chebi#59999</rdfs:seeAlso>
  </rdf:Description>
  <rdf:Description rdf:nodeID="nec5349e52cab421daaa8d343663bb464b1">
    <rdf:type rdf:resource="http://www.w3.org/2002/07/owl#Restriction"/>
    <owl:onProperty rdf:resource="http://w3id.org/CEON/ontology/material/hasChemicalEntity"/>
    <owl:someValuesFrom rdf:resource="http://w3id.org/CEON/ontology/material/ChemicalEntity"/>
  </rdf:Description>
  <rdf:Description rdf:about="http://w3id.org/CEON/ontology/material/ChemicalEntity">
    <rdf:type rdf:resource="http://www.w3.org/2002/07/owl#Class"/>
    <rdfs:subClassOf rdf:resource="http://w3id.org/CEON/ontology/resourceODP/Matter"/>
    <rdfs:comment>A chemical entity is an abstraction of entities that can compose matter. For instance, a chemical entity can be a molecular entity or a chemical substance.</rdfs:comment>
    <rdfs:label>Chemical Entity</rdfs:label>
    <rdfs:seeAlso>http://emmo.info/emmo#EMMO_47338839_6cca_4a8e_b565_3c4d5517e2c0</rdfs:seeAlso>
    <rdfs:seeAlso>http://purl.obolibrary.org/obo/chebi#24431</rdfs:seeAlso>
  </rdf:Description>
  <rdf:Description rdf:about="http://w3id.org/CEON/ontology/material/Copper">
    <rdf:type rdf:resource="http://www.w3.org/2002/07/owl#Class"/>
    <rdfs:subClassOf rdf:resource="http://w3id.org/CEON/ontology/material/ChemicalElement"/>
    <rdfs:comment>Copper is a chemical element with the symbol Cu and atomic number 29.</rdfs:comment>
    <rdfs:label>Copper</rdfs:label>
  </rdf:Description>
  <rdf:Description rdf:about="http://w3id.org/CEON/ontology/material/Promethium">
    <rdf:type rdf:resource="http://www.w3.org/2002/07/owl#Class"/>
    <rdfs:subClassOf rdf:resource="http://w3id.org/CEON/ontology/material/RareEarthElement"/>
    <rdfs:comment>Promethium is a chemical element with the symbol Pm and atomic number 61.</rdfs:comment>
    <rdfs:label>Promethium</rdfs:label>
  </rdf:Description>
  <rdf:Description rdf:about="http://w3id.org/CEON/ontology/material/Thulium">
    <rdf:type rdf:resource="http://www.w3.org/2002/07/owl#Class"/>
    <rdfs:subClassOf rdf:resource="http://w3id.org/CEON/ontology/material/RareEarthElement"/>
    <rdfs:comment>Thulium is a chemical element with the symbol Tm and atomic number 69.</rdfs:comment>
    <rdfs:label>Thulium</rdfs:label>
  </rdf:Description>
  <rdf:Description rdf:about="http://w3id.org/CEON/ontology/material/Yttrium">
    <rdf:type rdf:resource="http://www.w3.org/2002/07/owl#Class"/>
    <rdfs:subClassOf rdf:resource="http://w3id.org/CEON/ontology/material/RareEarthElement"/>
    <rdfs:comment>Yttrium is a chemical element with the symbol Y and atomic number 39.</rdfs:comment>
    <rdfs:label>Yttrium</rdfs:label>
  </rdf:Description>
  <rdf:Description rdf:about="http://w3id.org/CEON/ontology/material/MolecularEntity">
    <rdf:type rdf:resource="http://www.w3.org/2002/07/owl#Class"/>
    <rdfs:subClassOf rdf:resource="http://w3id.org/CEON/ontology/material/ChemicalEntity"/>
    <rdfs:comment>A molecular entity means a singular/distinguishable entity. It can be for instance, atom, ion.</rdfs:comment>
    <rdfs:label>Molecular Entity</rdfs:label>
    <rdfs:seeAlso>http://emmo.info/emmo#EMMO_21205421_5783_4d3e_81e5_10c5d894a88a</rdfs:seeAlso>
    <rdfs:seeAlso>http://purl.obolibrary.org/obo/chebi#23367</rdfs:seeAlso>
  </rdf:Description>
  <rdf:Description rdf:about="http://w3id.org/CEON/ontology/material/Chromium">
    <rdf:type rdf:resource="http://www.w3.org/2002/07/owl#Class"/>
    <rdfs:subClassOf rdf:resource="http://w3id.org/CEON/ontology/material/ChemicalElement"/>
    <rdfs:comment>Chromium is a chemical element with the symbol Cr and atomic number 24.</rdfs:comment>
    <rdfs:label>Chromium</rdfs:label>
  </rdf:Description>
  <rdf:Description rdf:about="http://w3id.org/CEON/ontology/material/Europium">
    <rdf:type rdf:resource="http://www.w3.org/2002/07/owl#Class"/>
    <rdfs:subClassOf rdf:resource="http://w3id.org/CEON/ontology/material/RareEarthElement"/>
    <rdfs:comment>Europium is a chemical element with the symbol Eu and atomic number 63.</rdfs:comment>
    <rdfs:label>Europium</rdfs:label>
  </rdf:Description>
  <rdf:Description rdf:about="http://w3id.org/CEON/ontology/material/">
    <rdf:type rdf:resource="http://www.w3.org/2002/07/owl#Ontology"/>
    <owl:versionIRI rdf:resource="http://w3id.org/CEON/ontology/material/0.4/"/>
    <owl:imports rdf:resource="http://w3id.org/CEON/ontology/resourceODP/0.5/"/>
    <dcterms:contributor>Eva Blomqvist</dcterms:contributor>
    <dcterms:contributor>Mikael Lindecrantz</dcterms:contributor>
    <dcterms:contributor>Robin Keskisärkkä</dcterms:contributor>
    <dcterms:created rdf:datatype="http://www.w3.org/2001/XMLSchema#date">2025-03-20</dcterms:created>
    <dcterms:issued rdf:datatype="http://www.w3.org/2001/XMLSchema#date">2025-06-30</dcterms:issued>
    <dcterms:publisher>Onto-DESIDE</dcterms:publisher>
    <dcterms:creator>Huanyu Li</dcterms:creator>
    <dcterms:description>The Material module of CEON (Circular Economy Ontology Network).</dcterms:description>
    <dcterms:license>https://creativecommons.org/licenses/by/4.0/</dcterms:license>
    <dcterms:title>Circular Economy Ontology Network (CEON) - Material Module</dcterms:title>
    <vann:preferredNamespacePrefix>ceon-material</vann:preferredNamespacePrefix>
    <vann:preferredNamespaceUri>http://w3id.org/CEON/ontology/material/</vann:preferredNamespaceUri>
    <odp:coversRequirements>In addition to requirements covered by imported ODPs, covers the following requirements from Onto-DESIDE D3.1: CVN-Resource-2, CVN-ResourceType-4, C3-3, E1-3, E2-4, E5-2, T1-1, T10-2.</odp:coversRequirements>
    <odp:coversRequirements>In addition to requirements covered by imported ODPs, covers the following requirements from Onto-DESIDE D3.2: CE5-2, C3-3, E1-3, E2-4, E5-2, T1-1, T10-2.</odp:coversRequirements>
    <rdfs:seeAlso rdf:resource="https://github.com/LiUSemWeb/CEON"/>
    <owl:priorVersion rdf:datatype="http://www.w3.org/2001/XMLSchema#decimal">0.3</owl:priorVersion>
    <owl:versionInfo rdf:datatype="http://www.w3.org/2001/XMLSchema#decimal">0.4</owl:versionInfo>
  </rdf:Description>
  <rdf:Description rdf:about="http://w3id.org/CEON/ontology/material/Praseodymium">
    <rdf:type rdf:resource="http://www.w3.org/2002/07/owl#Class"/>
    <rdfs:subClassOf rdf:resource="http://w3id.org/CEON/ontology/material/RareEarthElement"/>
    <rdfs:comment>Praseodymium is a chemical element with the symbol Pr and atomic number 59.</rdfs:comment>
    <rdfs:label>Praseodymium</rdfs:label>
  </rdf:Description>
  <rdf:Description rdf:about="http://w3id.org/CEON/ontology/material/Scandium">
    <rdf:type rdf:resource="http://www.w3.org/2002/07/owl#Class"/>
    <rdfs:subClassOf rdf:resource="http://w3id.org/CEON/ontology/material/RareEarthElement"/>
    <rdfs:comment>Scandium is a chemical element with the symbol Sc and atomic number 21.</rdfs:comment>
    <rdfs:label>Scandium</rdfs:label>
  </rdf:Description>
  <rdf:Description rdf:about="http://w3id.org/CEON/ontology/material/Terbium">
    <rdf:type rdf:resource="http://www.w3.org/2002/07/owl#Class"/>
    <rdfs:subClassOf rdf:resource="http://w3id.org/CEON/ontology/material/RareEarthElement"/>
    <rdfs:comment>Terbium is a chemical element with the symbol Tb and atomic number 65.</rdfs:comment>
    <rdfs:label>Terbium</rdfs:label>
  </rdf:Description>
  <rdf:Description rdf:about="http://w3id.org/CEON/ontology/material/Zinc">
    <rdf:type rdf:resource="http://www.w3.org/2002/07/owl#Class"/>
    <rdfs:subClassOf rdf:resource="http://w3id.org/CEON/ontology/material/ChemicalElement"/>
    <rdfs:comment>Zinc is a chemical element with the symbol Zn and atomic number 30.</rdfs:comment>
    <rdfs:label>Zinc</rdfs:label>
  </rdf:Description>
  <rdf:Description rdf:about="http://w3id.org/CEON/ontology/material/MaterialComponent">
    <rdf:type rdf:resource="http://www.w3.org/2002/07/owl#Class"/>
    <rdfs:subClassOf rdf:resource="http://w3id.org/CEON/ontology/resourceODP/Constituent"/>
    <rdfs:comment>A material component is a part of a material.</rdfs:comment>
    <rdfs:label>Material Component</rdfs:label>
  </rdf:Description>
  <rdf:Description rdf:about="http://w3id.org/CEON/ontology/material/Lutetium">
    <rdf:type rdf:resource="http://www.w3.org/2002/07/owl#Class"/>
    <rdfs:subClassOf rdf:resource="http://w3id.org/CEON/ontology/material/RareEarthElement"/>
    <rdfs:comment>Lutetium is a chemical element with the symbol Lu and atomic number 71.</rdfs:comment>
    <rdfs:label>Lutetium</rdfs:label>
  </rdf:Description>
  <rdf:Description rdf:about="http://w3id.org/CEON/ontology/material/Cellulose">
    <rdf:type rdf:resource="http://www.w3.org/2002/07/owl#Class"/>
    <rdfs:subClassOf rdf:resource="http://w3id.org/CEON/ontology/material/Material"/>
    <rdfs:comment>Cellulose is an organic compound with chemical formula (C6H10O5)n.</rdfs:comment>
    <rdfs:label>Cellulose</rdfs:label>
  </rdf:Description>
  <rdf:Description rdf:about="http://w3id.org/CEON/ontology/material/Holmium">
    <rdf:type rdf:resource="http://www.w3.org/2002/07/owl#Class"/>
    <rdfs:subClassOf rdf:resource="http://w3id.org/CEON/ontology/material/RareEarthElement"/>
    <rdfs:comment>Holmium is a chemical element with the symbol Ho and atomic number 67.</rdfs:comment>
    <rdfs:label>Holmium</rdfs:label>
  </rdf:Description>
  <rdf:Description rdf:about="http://w3id.org/CEON/ontology/material/hasChemicalEntity">
    <rdf:type rdf:resource="http://www.w3.org/2002/07/owl#ObjectProperty"/>
    <rdfs:domain rdf:resource="http://w3id.org/CEON/ontology/material/Material"/>
    <rdfs:range rdf:resource="http://w3id.org/CEON/ontology/material/ChemicalEntity"/>
    <rdfs:comment>hasChemicalEntity intends to represent that a material can have a collection of chemical entities.</rdfs:comment>
    <rdfs:label>has chemical entity</rdfs:label>
  </rdf:Description>
  <rdf:Description rdf:about="http://w3id.org/CEON/ontology/material/anonymousFormula">
    <rdf:type rdf:resource="http://www.w3.org/2002/07/owl#DatatypeProperty"/>
    <rdfs:comment>anonymousFormula represents that a molecular entity has the anonymous formula in a string.</rdfs:comment>
    <rdfs:label>anonymous formula</rdfs:label>
    <rdfs:seeAlso>https://w3id.org/mdo/structure/AnonymousFormula</rdfs:seeAlso>
  </rdf:Description>
  <rdf:Description rdf:about="http://w3id.org/CEON/ontology/material/ChemicalElement">
    <rdf:type rdf:resource="http://www.w3.org/2002/07/owl#Class"/>
    <rdfs:subClassOf rdf:resource="http://w3id.org/CEON/ontology/material/ChemicalSubstance"/>
    <rdfs:comment>A chemical element is a chemical substance whose atoms all have the same number of protons.</rdfs:comment>
    <rdfs:label>Chemical Element</rdfs:label>
  </rdf:Description>
  <rdf:Description rdf:about="http://w3id.org/CEON/ontology/material/Nickel">
    <rdf:type rdf:resource="http://www.w3.org/2002/07/owl#Class"/>
    <rdfs:subClassOf rdf:resource="http://w3id.org/CEON/ontology/material/ChemicalElement"/>
    <rdfs:comment>Nickel is a chemical element with the symbol Ni and atomic number 28.</rdfs:comment>
    <rdfs:label>Nickel</rdfs:label>
  </rdf:Description>
  <rdf:Description rdf:about="http://w3id.org/CEON/ontology/material/descriptiveFormula">
    <rdf:type rdf:resource="http://www.w3.org/2002/07/owl#DatatypeProperty"/>
    <rdfs:comment>descriptiveFormula represents that a molecular entity has the descriptive formula in a string.</rdfs:comment>
    <rdfs:label>descriptive formula</rdfs:label>
    <rdfs:seeAlso>https://w3id.org/mdo/structure/DescriptiveFormula</rdfs:seeAlso>
  </rdf:Description>
  <rdf:Description rdf:about="http://w3id.org/CEON/ontology/material/Erbium">
    <rdf:type rdf:resource="http://www.w3.org/2002/07/owl#Class"/>
    <rdfs:subClassOf rdf:resource="http://w3id.org/CEON/ontology/material/RareEarthElement"/>
    <rdfs:comment>Erbium is a chemical element with the symbol Er and atomic number 68.</rdfs:comment>
    <rdfs:label>Erbium</rdfs:label>
  </rdf:Description>
  <rdf:Description rdf:about="http://w3id.org/CEON/ontology/resourceODP/Constituent">
    <rdf:type rdf:resource="http://www.w3.org/2002/07/owl#Class"/>
  </rdf:Description>
  <rdf:Description rdf:about="http://w3id.org/CEON/ontology/material/Material">
    <rdf:type rdf:resource="http://www.w3.org/2002/07/owl#Class"/>
    <rdfs:subClassOf rdf:resource="http://w3id.org/CEON/ontology/resourceODP/Matter"/>
    <rdfs:subClassOf rdf:nodeID="nec5349e52cab421daaa8d343663bb464b1"/>
    <rdfs:comment>Material as a sub-concept of Matter, can be a substance or a collection of substance which a physical object is composed of.</rdfs:comment>
    <rdfs:label>Material</rdfs:label>
    <rdfs:seeAlso>http://emmo.info/emmo#EMMO_4207e895_8b83_4318_996a_72cfb32acd94</rdfs:seeAlso>
    <rdfs:seeAlso>https://w3id.org/mdo/core/Material</rdfs:seeAlso>
  </rdf:Description>
  <rdf:Description rdf:about="http://w3id.org/CEON/ontology/material/reducedChemicalFormula">
    <rdf:type rdf:resource="http://www.w3.org/2002/07/owl#DatatypeProperty"/>
    <rdfs:comment>reducedChemicalFormula represents that a molecular entity has the reduced chemical formula in a string.</rdfs:comment>
    <rdfs:label>reduced chemical formula</rdfs:label>
    <rdfs:seeAlso>https://w3id.org/mdo/structure/ReducedFormula</rdfs:seeAlso>
  </rdf:Description>
  <rdf:Description rdf:about="http://w3id.org/CEON/ontology/material/Neodymium">
    <rdf:type rdf:resource="http://www.w3.org/2002/07/owl#Class"/>
    <rdfs:subClassOf rdf:resource="http://w3id.org/CEON/ontology/material/RareEarthElement"/>
    <rdfs:comment>Neodymium is a chemical element with the symbol Nd and atomic number 60.</rdfs:comment>
    <rdfs:label>Neodymium</rdfs:label>
  </rdf:Description>
  <rdf:Description rdf:about="http://w3id.org/CEON/ontology/material/hasMaterialComponent">
    <rdf:type rdf:resource="http://www.w3.org/2002/07/owl#ObjectProperty"/>
    <rdfs:domain rdf:resource="http://w3id.org/CEON/ontology/material/Material"/>
    <rdfs:range rdf:resource="http://w3id.org/CEON/ontology/material/MaterialComponent"/>
    <rdfs:comment>hasMaterialComponent intends to represent that a material can have a collection of components.</rdfs:comment>
    <rdfs:label>has material component</rdfs:label>
  </rdf:Description>
  <rdf:Description rdf:about="http://w3id.org/CEON/ontology/material/RareEarthElement">
    <rdf:type rdf:resource="http://www.w3.org/2002/07/owl#Class"/>
    <rdfs:subClassOf rdf:resource="http://w3id.org/CEON/ontology/material/ChemicalElement"/>
    <rdfs:comment>Rare earth elements is a set of 17 nearly indistinguishable lustrous silvery-white soft heavy metals.</rdfs:comment>
    <rdfs:label>Rare Earth Element</rdfs:label>
  </rdf:Description>
  <rdf:Description rdf:about="http://w3id.org/CEON/ontology/material/Niobium">
    <rdf:type rdf:resource="http://www.w3.org/2002/07/owl#Class"/>
    <rdfs:subClassOf rdf:resource="http://w3id.org/CEON/ontology/material/ChemicalElement"/>
    <rdfs:comment>Niobium is a chemical element with the symbol Nb and atomic number 41.</rdfs:comment>
    <rdfs:label>Niobium</rdfs:label>
  </rdf:Description>
  <rdf:Description rdf:about="http://w3id.org/CEON/ontology/material/Manganese">
    <rdf:type rdf:resource="http://www.w3.org/2002/07/owl#Class"/>
    <rdfs:subClassOf rdf:resource="http://w3id.org/CEON/ontology/material/ChemicalElement"/>
    <rdfs:comment>Manganese is a chemical element with the symbol Mn and atomic number 25.</rdfs:comment>
    <rdfs:label>Manganese</rdfs:label>
  </rdf:Description>
  <rdf:Description rdf:about="http://w3id.org/CEON/ontology/material/Gadolinium">
    <rdf:type rdf:resource="http://www.w3.org/2002/07/owl#Class"/>
    <rdfs:subClassOf rdf:resource="http://w3id.org/CEON/ontology/material/RareEarthElement"/>
    <rdfs:comment>Gadolinium is a chemical element with the symbol Gd and atomic number 64.</rdfs:comment>
    <rdfs:label>Gadolinium</rdfs:label>
  </rdf:Description>
  <rdf:Description rdf:about="http://w3id.org/CEON/ontology/material/Samarium">
    <rdf:type rdf:resource="http://www.w3.org/2002/07/owl#Class"/>
    <rdfs:subClassOf rdf:resource="http://w3id.org/CEON/ontology/material/RareEarthElement"/>
    <rdfs:comment>Samarium is a chemical element with the symbol Sm and atomic number 62.</rdfs:comment>
    <rdfs:label>Samarium</rdfs:label>
  </rdf:Description>
  <rdf:Description rdf:about="http://w3id.org/CEON/ontology/material/Boron">
    <rdf:type rdf:resource="http://www.w3.org/2002/07/owl#Class"/>
    <rdfs:subClassOf rdf:resource="http://w3id.org/CEON/ontology/material/ChemicalElement"/>
    <rdfs:comment>Boron is a chemical element with the symbol B and atomic number 5.</rdfs:comment>
    <rdfs:label>Boron</rdfs:label>
  </rdf:Description>
  <rdf:Description rdf:about="http://w3id.org/CEON/ontology/material/Silicon">
    <rdf:type rdf:resource="http://www.w3.org/2002/07/owl#Class"/>
    <rdfs:subClassOf rdf:resource="http://w3id.org/CEON/ontology/material/ChemicalElement"/>
    <rdfs:comment>Silicon is a chemical element with the symbol Si and atomic number 14.</rdfs:comment>
    <rdfs:label>Silicon</rdfs:label>
  </rdf:Description>
  <rdf:Description rdf:about="http://w3id.org/CEON/ontology/material/hillFormula">
    <rdf:type rdf:resource="http://www.w3.org/2002/07/owl#DatatypeProperty"/>
    <rdfs:comment>hillFormula represents that a composition has the hill formula in a string.</rdfs:comment>
    <rdfs:label>hill formula</rdfs:label>
    <rdfs:seeAlso>https://w3id.org/mdo/structure/HillFormula</rdfs:seeAlso>
  </rdf:Description>
  <rdf:Description rdf:about="http://w3id.org/CEON/ontology/material/Iron">
    <rdf:type rdf:resource="http://www.w3.org/2002/07/owl#Class"/>
    <rdfs:subClassOf rdf:resource="http://w3id.org/CEON/ontology/material/ChemicalElement"/>
    <rdfs:comment>Iron is a chemical element with the symbol Fe and atomic number 26.</rdfs:comment>
    <rdfs:label>Iron</rdfs:label>
  </rdf:Description>
  <rdf:Description rdf:about="http://w3id.org/CEON/ontology/material/Tantalum">
    <rdf:type rdf:resource="http://www.w3.org/2002/07/owl#Class"/>
    <rdfs:subClassOf rdf:resource="http://w3id.org/CEON/ontology/material/RareEarthElement"/>
    <rdfs:comment>Tantalum is a chemical element with the symbol Ta and atomic number 73.</rdfs:comment>
    <rdfs:label>Tantalum</rdfs:label>
  </rdf:Description>
  <rdf:Description rdf:about="http://w3id.org/CEON/ontology/resourceODP/Matter">
    <rdf:type rdf:resource="http://www.w3.org/2002/07/owl#Class"/>
  </rdf:Description>
  <rdf:Description rdf:about="http://w3id.org/CEON/ontology/material/Titanium">
    <rdf:type rdf:resource="http://www.w3.org/2002/07/owl#Class"/>
    <rdfs:subClassOf rdf:resource="http://w3id.org/CEON/ontology/material/ChemicalElement"/>
    <rdfs:comment>Titanium is a chemical element with the symbol Ti and atomic number 22.</rdfs:comment>
    <rdfs:label>Titanium</rdfs:label>
  </rdf:Description>
</rdf:RDF>
