@prefix : <http://w3id.org/CEON/ontology/product/> .
@prefix dc: <http://purl.org/dc/elements/1.1/> .
@prefix odp: <http://www.ontologydesignpatterns.org/schemas/cpannotationschema.owl#> .
@prefix owl: <http://www.w3.org/2002/07/owl#> .
@prefix rdf: <http://www.w3.org/1999/02/22-rdf-syntax-ns#> .
@prefix xml: <http://www.w3.org/XML/1998/namespace> .
@prefix xsd: <http://www.w3.org/2001/XMLSchema#> .
@prefix rdfs: <http://www.w3.org/2000/01/rdf-schema#> .
@prefix vann: <http://purl.org/vocab/vann/> .
@prefix dcterms: <http://purl.org/dc/terms/> .
@prefix actorODP: <http://w3id.org/CEON/ontology/actorODP/> .
@prefix resourceODP: <http://w3id.org/CEON/ontology/resourceODP/> .
@base <http://w3id.org/CEON/ontology/product/> .

<http://w3id.org/CEON/ontology/product/> rdf:type owl:Ontology ;
                                          owl:versionIRI <http://w3id.org/CEON/ontology/product/0.4/> ;
                                          owl:imports <http://w3id.org/CEON/ontology/actorODP/0.3/> ,
                                                      <http://w3id.org/CEON/ontology/resourceODP/0.3/> ;
                                          dcterms:contributor "Eva Blomqvist" ,
                                                              "Mikael Lindecrantz" ,
                                                              "Robin Keskisärkkä" ;
                                          dcterms:created "2023-03-16" ;
                                          dcterms:creator "Huanyu Li" ;
                                          dcterms:description "The Product module of CEON (Circular Economy Ontology Network)." ;
                                          dcterms:license "https://creativecommons.org/licenses/by/4.0/" ;
                                          dcterms:title "Circular Economy Ontology Network (CEON) - Product Module" ;
                                          vann:preferredNamespacePrefix "product" ;
                                          vann:preferredNamespaceUri "http://w3id.org/CEON/ontology/product/" ;
                                          odp:coversRequirements "In addition to requirements covered by imported ODPs, covers the following requirements from Onto-DESIDE D3.1: CVN-Resource-2, CVN-ResrouceType-4, C11-2, C12-1, C13-3, E2-1, T8-3." ;
                                          rdfs:seeAlso <https://github.com/LiUSemWeb/CEON> ;
                                          owl:versionInfo 0.4 .

#################################################################
#    Annotation properties
#################################################################

###  http://purl.org/dc/terms/contributor
dcterms:contributor rdf:type owl:AnnotationProperty .


###  http://purl.org/dc/terms/created
dcterms:created rdf:type owl:AnnotationProperty .


###  http://purl.org/dc/terms/creator
dcterms:creator rdf:type owl:AnnotationProperty .


###  http://purl.org/dc/terms/description
dcterms:description rdf:type owl:AnnotationProperty .


###  http://purl.org/dc/terms/license
dcterms:license rdf:type owl:AnnotationProperty .


###  http://purl.org/dc/terms/title
dcterms:title rdf:type owl:AnnotationProperty .


###  http://purl.org/vocab/vann/preferredNamespacePrefix
vann:preferredNamespacePrefix rdf:type owl:AnnotationProperty .


###  http://purl.org/vocab/vann/preferredNamespaceUri
vann:preferredNamespaceUri rdf:type owl:AnnotationProperty .


###  http://www.ontologydesignpatterns.org/schemas/cpannotationschema.owl#coversRequirements
odp:coversRequirements rdf:type owl:AnnotationProperty .


#################################################################
#    Object Properties
#################################################################

###  http://w3id.org/CEON/ontology/product/associatedWithMatter
:associatedWithMatter rdf:type owl:ObjectProperty ;
                      rdfs:domain :MatterComposition ;
                      rdfs:range resourceODP:Matter ;
                      rdfs:comment "associatedWithMatter intends to represent the matter to which a matter compopsition information regards to."@en ;
                      rdfs:label "associated with matter"@en .


###  http://w3id.org/CEON/ontology/product/associatedWithProductModel
:associatedWithProductModel rdf:type owl:ObjectProperty ;
                            rdfs:domain :ProductComposition ;
                            rdfs:range :Product ;
                            rdfs:comment "associatedWithProductModel intends to represent the product model to which a product compopsition information regards to."@en ;
                            rdfs:label "associated with product model"@en .


###  http://w3id.org/CEON/ontology/product/associatedWithProductObject
:associatedWithProductObject rdf:type owl:ObjectProperty ;
                             rdfs:subPropertyOf owl:topObjectProperty ;
                             rdfs:domain :ProductObjectComposition ;
                             rdfs:range :Item ;
                             rdfs:comment "associatedWithProductObject intends to represent the item (product object) to which a product object compopsition information regards to." ;
                             rdfs:label "associated with product object" .


###  http://w3id.org/CEON/ontology/product/batchOfProduct
:batchOfProduct rdf:type owl:ObjectProperty ;
                rdfs:domain resourceODP:BatchOfObjects ;
                rdfs:range :Product ;
                rdfs:comment "batchOfProduct intends to represent what is the model product of a batch of objects."@en ;
                rdfs:label "batch of products"@en .


###  http://w3id.org/CEON/ontology/product/complianceWith
:complianceWith rdf:type owl:ObjectProperty ;
                rdfs:domain :Compliance ;
                rdfs:comment "Represents what the compliance is compliant with (e.g. a standard or regulation)." ;
                rdfs:label "Compliance with" .


###  http://w3id.org/CEON/ontology/product/compositionOf
:compositionOf rdf:type owl:ObjectProperty ;
               rdfs:domain resourceODP:Composition ;
               rdfs:range [ rdf:type owl:Class ;
                            owl:unionOf ( :Item
                                          :Product
                                          resourceODP:Matter
                                        )
                          ] ;
               rdfs:comment "Represents what the composition is a composition of (i.e., the product, the product object or matter that is broken down into its components)." ;
               rdfs:label "composition of" .


###  http://w3id.org/CEON/ontology/product/hasCompliance
:hasCompliance rdf:type owl:ObjectProperty ;
               rdfs:domain [ rdf:type owl:Class ;
                             owl:unionOf ( actorODP:Actor
                                           <http://w3id.org/CEON/ontology/processODP/Process>
                                           :Item
                                           :Product
                                         )
                           ] ;
               rdfs:range :Compliance ;
               rdfs:comment "Used to link something (e.g., product or process) to a compliance." ;
               rdfs:label "has compliance" .


###  http://w3id.org/CEON/ontology/product/hasComposition
:hasComposition rdf:type owl:ObjectProperty ;
                rdfs:domain [ rdf:type owl:Class ;
                              owl:unionOf ( :Product
                                            resourceODP:PhysicalObject
                                          )
                            ] ;
                rdfs:range resourceODP:Composition ;
                rdfs:comment "hasComposition intends to represent that a product model or physical object can have compostition information."@en ;
                rdfs:label "has composition" .


###  http://w3id.org/CEON/ontology/product/hasProductComponent
:hasProductComponent rdf:type owl:ObjectProperty ;
                     rdfs:domain :Product ;
                     rdfs:range :Product ;
                     rdfs:comment "hasProductComponent intends to represent that a product can have other product components."@en ;
                     rdfs:label "has product component"@en .


###  http://w3id.org/CEON/ontology/product/hasProductObjectComponent
:hasProductObjectComponent rdf:type owl:ObjectProperty ;
                           rdfs:domain :Item ;
                           rdfs:range :Item ;
                           rdfs:label "has product object component" .


###  http://w3id.org/CEON/ontology/product/modelledBy
:modelledBy rdf:type owl:ObjectProperty ;
            rdfs:domain :Item ;
            rdfs:range :Product ;
            rdfs:comment "modelledBy intends to represent that product objects follow particular product models."@en ;
            rdfs:label "modelled by"@en .


#################################################################
#    Data properties
#################################################################

###  http://w3id.org/CEON/ontology/product/compositionQuantity
:compositionQuantity rdf:type owl:DatatypeProperty ;
                     rdfs:domain resourceODP:Composition ;
                     rdfs:range xsd:double ;
                     rdfs:comment "compositionQuantity represents the quantity of elements of a composition." ;
                     rdfs:label "Composition quantity"@en .


###  http://w3id.org/CEON/ontology/product/countryOfAssembly
:countryOfAssembly rdf:type owl:DatatypeProperty ;
                   rdfs:subPropertyOf :locationOfAssembly ;
                   rdfs:comment "Used to represent the country of assembly of a product or product object" ;
                   rdfs:label "Country of assembly" .


###  http://w3id.org/CEON/ontology/product/countryOfManufacture
:countryOfManufacture rdf:type owl:DatatypeProperty ;
                      rdfs:subPropertyOf :locationOfManufacture ;
                      rdfs:comment "Used to represent the country of manufacture of a product or product object" ;
                      rdfs:label "Country of manufacture" .


###  http://w3id.org/CEON/ontology/product/countryOfOrigin
:countryOfOrigin rdf:type owl:DatatypeProperty ;
                 rdfs:subPropertyOf :locationOfOrigin ;
                 rdfs:comment "Used to represent the country of origin of a product or product object" ;
                 rdfs:label "Country of origin" .


###  http://w3id.org/CEON/ontology/product/hasCertificate
:hasCertificate rdf:type owl:DatatypeProperty ;
                rdfs:domain :Compliance ;
                rdfs:comment "Link to the the certificate that certifies the compliance" ;
                rdfs:label "has certificate" .


###  http://w3id.org/CEON/ontology/product/locationOfAssembly
:locationOfAssembly rdf:type owl:DatatypeProperty ;
                    rdfs:domain [ rdf:type owl:Class ;
                                  owl:unionOf ( :Item
                                                :Product
                                              )
                                ] ;
                    rdfs:range xsd:string ;
                    rdfs:comment "Used to represent the location of assembly of a product or product object" ;
                    rdfs:label "Location of assembly" .


###  http://w3id.org/CEON/ontology/product/locationOfManufacture
:locationOfManufacture rdf:type owl:DatatypeProperty ;
                       rdfs:domain [ rdf:type owl:Class ;
                                     owl:unionOf ( :Item
                                                   :Product
                                                 )
                                   ] ;
                       rdfs:range xsd:string ;
                       rdfs:comment "Used to represent the location of manufacture of a product or product object" ;
                       rdfs:label "Location of manufacture" .


###  http://w3id.org/CEON/ontology/product/locationOfOrigin
:locationOfOrigin rdf:type owl:DatatypeProperty ;
                  rdfs:domain [ rdf:type owl:Class ;
                                owl:unionOf ( :Item
                                              :Product
                                            )
                              ] ;
                  rdfs:range xsd:string ;
                  rdfs:comment "Used to represent the location of origin of a product or product object" ;
                  rdfs:label "Location of origin" .


#################################################################
#    Classes
#################################################################

###  http://w3id.org/CEON/ontology/actorODP/Actor
actorODP:Actor rdf:type owl:Class .


###  http://w3id.org/CEON/ontology/actorODP/ResourceRelation
actorODP:ResourceRelation rdf:type owl:Class .


###  http://w3id.org/CEON/ontology/processODP/Process
<http://w3id.org/CEON/ontology/processODP/Process> rdf:type owl:Class .


###  http://w3id.org/CEON/ontology/product/Compliance
:Compliance rdf:type owl:Class ;
            rdfs:comment "Represents that something is compliant with some standard or has a received a certain certification." ;
            rdfs:label "Compliance" .


###  http://w3id.org/CEON/ontology/product/Item
:Item rdf:type owl:Class ;
      rdfs:subClassOf resourceODP:PhysicalObject ,
                      [ rdf:type owl:Restriction ;
                        owl:onProperty :modelledBy ;
                        owl:qualifiedCardinality "1"^^xsd:nonNegativeInteger ;
                        owl:onClass :Product
                      ] ;
      rdfs:comment "An item is a physical object put into a market for sale, i.e. corresponding to an individual of a product. The item can be a thing that grows naturally or produced through some chemical or manufacturing processes."@en ;
      rdfs:label "Item"@en .


###  http://w3id.org/CEON/ontology/product/MatterComposition
:MatterComposition rdf:type owl:Class ;
                   rdfs:subClassOf resourceODP:Composition ,
                                   [ rdf:type owl:Restriction ;
                                     owl:onProperty :associatedWithMatter ;
                                     owl:qualifiedCardinality "1"^^xsd:nonNegativeInteger ;
                                     owl:onClass resourceODP:Matter
                                   ] ;
                   rdfs:comment "A product composition is the composed information of a product in terms of a specific component, in which such a component is also a matter."@en ;
                   rdfs:label "Matter composition"@en .


###  http://w3id.org/CEON/ontology/product/Product
:Product rdf:type owl:Class ;
         rdfs:subClassOf :Solution ,
                         [ rdf:type owl:Restriction ;
                           owl:onProperty :hasComposition ;
                           owl:someValuesFrom :MatterComposition
                         ] ,
                         [ rdf:type owl:Restriction ;
                           owl:onProperty :hasComposition ;
                           owl:someValuesFrom :ProductComposition
                         ] ;
         rdfs:comment "Represents the common sense notion of a product, i.e. the abstract notion of a product type, which is a model that is used for manufacturing items of that product."@en ;
         rdfs:label "Product"@en .


###  http://w3id.org/CEON/ontology/product/ProductComposition
:ProductComposition rdf:type owl:Class ;
                    rdfs:subClassOf resourceODP:Composition ,
                                    [ rdf:type owl:Restriction ;
                                      owl:onProperty :associatedWithProductModel ;
                                      owl:qualifiedCardinality "1"^^xsd:nonNegativeInteger ;
                                      owl:onClass :Product
                                    ] ;
                    rdfs:comment "A product composition is the composed information of a product in terms of a specific component, in which such a component is also a product."@en ;
                    rdfs:label "Product composition"@en .


###  http://w3id.org/CEON/ontology/product/ProductObjectComposition
:ProductObjectComposition rdf:type owl:Class ;
                          rdfs:subClassOf resourceODP:Composition ,
                                          [ rdf:type owl:Restriction ;
                                            owl:onProperty :associatedWithProductObject ;
                                            owl:qualifiedCardinality "1"^^xsd:nonNegativeInteger ;
                                            owl:onClass :Item
                                          ] ;
                          rdfs:comment "A product object composition is the composed information of a product object in terms of a specific component, in which such a component is also a product object." ;
                          rdfs:label "Product Object Composition" .


###  http://w3id.org/CEON/ontology/product/Solution
:Solution rdf:type owl:Class ;
          rdfs:comment "Product or service, or a combination thereof, that fulfils a need of an interested party."@en ;
          rdfs:label "Solution"@en ;
          <http://www.w3.org/2004/02/skos/core#definition> "ISO 59004:2024 - 3.2.1 solution" .


###  http://w3id.org/CEON/ontology/resourceODP/BatchOfObjects
resourceODP:BatchOfObjects rdf:type owl:Class ;
                           rdfs:subClassOf [ rdf:type owl:Restriction ;
                                             owl:onProperty :batchOfProduct ;
                                             owl:qualifiedCardinality "1"^^xsd:nonNegativeInteger ;
                                             owl:onClass :Product
                                           ] .


###  http://w3id.org/CEON/ontology/resourceODP/Composition
resourceODP:Composition rdf:type owl:Class ;
                        rdfs:subClassOf actorODP:ResourceRelation .


###  http://w3id.org/CEON/ontology/resourceODP/Matter
resourceODP:Matter rdf:type owl:Class .


###  http://w3id.org/CEON/ontology/resourceODP/PhysicalObject
resourceODP:PhysicalObject rdf:type owl:Class .


###  Generated by the OWL API (version 4.5.25.2023-02-15T19:15:49Z) https://github.com/owlcs/owlapi
