@prefix : <http://w3id.org/CEON/ontology/processODP/> .
@prefix dcterms: <http://purl.org/dc/terms/> .
@prefix odp: <http://www.ontologydesignpatterns.org/schemas/cpannotationschema.owl#> .
@prefix owl: <http://www.w3.org/2002/07/owl#> .
@prefix rdfs: <http://www.w3.org/2000/01/rdf-schema#> .
@prefix vann: <http://purl.org/vocab/vann/> .
@prefix xsd: <http://www.w3.org/2001/XMLSchema#> .

dcterms:contributor a owl:AnnotationProperty .

dcterms:created a owl:AnnotationProperty .

dcterms:creator a owl:AnnotationProperty .

dcterms:description a owl:AnnotationProperty .

dcterms:license a owl:AnnotationProperty .

dcterms:title a owl:AnnotationProperty .

vann:preferredNamespacePrefix a owl:AnnotationProperty .

vann:preferredNamespaceUri a owl:AnnotationProperty .

: a owl:Ontology ;
    dcterms:contributor "Eva Blomqvist",
        "Mikael Lindecrantz",
        "Robin Keskisärkkä" ;
    dcterms:created "2024-11-13" ;
    dcterms:creator "Huanyu Li" ;
    dcterms:description "A core ODP of the CEON ontology network, defining aspects of the process concept." ;
    dcterms:license "https://creativecommons.org/licenses/by/4.0/" ;
    dcterms:title "Circular Economy Ontology Network (CEON) - Process ODP" ;
    vann:preferredNamespacePrefix "processODP" ;
    vann:preferredNamespaceUri "http://w3id.org/CEON/ontology/processODP/" ;
    odp:coversRequirements "Covers the following requirements from Onto-DESIDE D3.1: CVN-Process-3,4,5, C3-1, C4-2, C4-5, C4-7, C4-9, C13-2, E2-6" ;
    rdfs:comment "A core ODP of the CEON ontology network, defining aspects of the process concept." ;
    rdfs:seeAlso <https://github.com/LiUSemWeb/CEON> ;
    owl:versionIRI <http://w3id.org/CEON/ontology/processODP/0.3/> ;
    owl:versionInfo 0.3 .

:hasInput a owl:ObjectProperty ;
    rdfs:label "has input" ;
    rdfs:comment "The situation before the process has an execution, i.e. the state of affairs before the process takes places, such as the set of components before they are assembled into a product." ;
    rdfs:domain :Process .

:hasOutput a owl:ObjectProperty ;
    rdfs:label "has output" ;
    rdfs:comment "The output situation of after the process is executed, i.e. the state of affairs after the process is executed." ;
    rdfs:domain :Process .

:hasPart a owl:ObjectProperty,
        owl:TransitiveProperty ;
    rdfs:label "has part" ;
    rdfs:comment "A process can consists of several part, which are sub-processes." ;
    rdfs:domain :Process ;
    rdfs:range :Process .

:hasProcessType a owl:ObjectProperty ;
    rdfs:label "has process type" ;
    rdfs:comment "The type of the process." ;
    rdfs:domain :Process ;
    rdfs:range :ProcessType .

:intialSituation a owl:ObjectProperty ;
    rdfs:label "initial situation" ;
    rdfs:comment "The situation before executing a process." ;
    rdfs:domain :ProcessExecution ;
    rdfs:range :Situation .

:nextExecution a owl:ObjectProperty ;
    rdfs:label "next execution" ;
    rdfs:comment "A relation between one execution and the next one following it in some sequence of executions, e.g. a sequence of transformations in a material flow." ;
    rdfs:domain :ProcessExecution ;
    rdfs:range :ProcessExecution .

:nextProcess a owl:ObjectProperty ;
    rdfs:label "next process" ;
    rdfs:comment "A relation between one process and the next one following it in some sequence of processes, e.g. a sequence of transformations in a material flow." ;
    rdfs:domain :Process ;
    rdfs:range :Process .

:occursAtLocation a owl:ObjectProperty ;
    rdfs:label "occurs at location" ;
    rdfs:comment "The location in which an execution takes place, e.g. the factory location where something is manufactured." ;
    rdfs:domain :ProcessExecution .

:occursAtTime a owl:DatatypeProperty ;
    rdfs:label "occurs at time" ;
    rdfs:comment "Represents the time at which something takes place." ;
    rdfs:domain :ProcessExecution ;
    rdfs:range xsd:dateTime .

:resultingSituation a owl:ObjectProperty ;
    rdfs:label "resulting situation" ;
    rdfs:comment "The situation after the execution of a process." ;
    rdfs:domain :ProcessExecution ;
    rdfs:range :Situation .

odp:coversRequirements a owl:AnnotationProperty .

:ProcessType a owl:Class ;
    rdfs:label "Process type" ;
    rdfs:comment "The type of a process." .

:Transformation a owl:Class ;
    rdfs:label "Transformation" ;
    rdfs:comment "A process that transforms some situation into another situation, i.e. changes the state of affairs of some actor, resource etc." ;
    rdfs:subClassOf [ a owl:Restriction ;
            owl:onProperty :hasTransformationExecution ;
            owl:someValuesFrom :TransformationExecution ],
        :Process .

:hasExecutionInput a owl:ObjectProperty ;
    rdfs:label "has execution input" ;
    rdfs:comment "The situation before the execution takes place, i.e. the state of affairs before the process takes places, such as the set of components before they are assembled into a product object." ;
    rdfs:domain :ProcessExecution .

:hasExecutionOutput a owl:ObjectProperty ;
    rdfs:label "has execution output" ;
    rdfs:comment "The situation after the execution takes place, i.e. the state of affairs before the process takes places, such as the assembled product object." ;
    rdfs:domain :ProcessExecution .

:hasTransformationExecution a owl:ObjectProperty ;
    rdfs:label "has transformation execution" ;
    rdfs:comment "A transformation can have specific transformation executions." ;
    rdfs:domain :Transformation ;
    rdfs:range :TransformationExecution ;
    rdfs:subPropertyOf :hasProcessExecution .

:isSettingFor a owl:ObjectProperty ;
    rdfs:label "is the setting for" ;
    rdfs:comment "The thing(s) that this situation is the setting for, e.g. a resource that is in a certain state." ;
    rdfs:domain :Situation .

:TransformationExecution a owl:Class ;
    rdfs:label "Transformation execution" ;
    rdfs:comment "An execution of a specific transformation at a specific location and time point or period." ;
    rdfs:subClassOf :ProcessExecution .

:hasProcessExecution a owl:ObjectProperty ;
    rdfs:label "has process execution"@en ;
    rdfs:comment "A process can have specific executions."@en ;
    rdfs:domain :Process ;
    rdfs:range :ProcessExecution .

:Situation a owl:Class ;
    rdfs:label "Situation" ;
    rdfs:comment "A situation that may involve some resources and actors, i.e. a state of affairs at a certain point in time." ;
    rdfs:subClassOf [ a owl:Restriction ;
            owl:onProperty :isSettingFor ;
            owl:someValuesFrom owl:Thing ] .

:Process a owl:Class ;
    rdfs:label "Process" ;
    rdfs:comment "An activity in the context of a circular value network, handling resources." ;
    rdfs:subClassOf [ a owl:Restriction ;
            owl:onProperty :hasProcessExecution ;
            owl:someValuesFrom :ProcessExecution ] .

:ProcessExecution a owl:Class ;
    rdfs:label "Process execution" ;
    rdfs:comment "An execution of a specific process at a specific location and time point." ;
    rdfs:subClassOf [ a owl:Restriction ;
            owl:onProperty :hasExecutionInput ;
            owl:someValuesFrom owl:Thing ],
        [ a owl:Restriction ;
            owl:onProperty :hasExecutionOutput ;
            owl:someValuesFrom owl:Thing ] .

