<?xml version="1.0" encoding="utf-8"?>
<rdf:RDF
   xmlns:dcterms="http://purl.org/dc/terms/"
   xmlns:odp="http://www.ontologydesignpatterns.org/schemas/cpannotationschema.owl#"
   xmlns:owl="http://www.w3.org/2002/07/owl#"
   xmlns:rdf="http://www.w3.org/1999/02/22-rdf-syntax-ns#"
   xmlns:rdfs="http://www.w3.org/2000/01/rdf-schema#"
   xmlns:vann="http://purl.org/vocab/vann/"
>
  <rdf:Description rdf:about="http://w3id.org/CEON/ontology/processODP/TransformationExecution">
    <rdf:type rdf:resource="http://www.w3.org/2002/07/owl#Class"/>
    <rdfs:subClassOf rdf:resource="http://w3id.org/CEON/ontology/processODP/ProcessExecution"/>
    <rdfs:comment>An execution of a specific transformation at a specific location and time point or period.</rdfs:comment>
    <rdfs:label>Transformation execution</rdfs:label>
  </rdf:Description>
  <rdf:Description rdf:about="http://w3id.org/CEON/ontology/processODP/hasTransformationExecution">
    <rdf:type rdf:resource="http://www.w3.org/2002/07/owl#ObjectProperty"/>
    <rdfs:subPropertyOf rdf:resource="http://w3id.org/CEON/ontology/processODP/hasProcessExecution"/>
    <rdfs:domain rdf:resource="http://w3id.org/CEON/ontology/processODP/Transformation"/>
    <rdfs:range rdf:resource="http://w3id.org/CEON/ontology/processODP/TransformationExecution"/>
    <rdfs:comment>A transformation can have specific transformation executions.</rdfs:comment>
    <rdfs:label>has transformation execution</rdfs:label>
  </rdf:Description>
  <rdf:Description rdf:about="http://w3id.org/CEON/ontology/processODP/occursAtLocation">
    <rdf:type rdf:resource="http://www.w3.org/2002/07/owl#ObjectProperty"/>
    <rdfs:domain rdf:resource="http://w3id.org/CEON/ontology/processODP/ProcessExecution"/>
    <rdfs:range rdf:resource="http://w3id.org/CEON/ontology/location/Location"/>
    <rdfs:comment>The location in which an execution takes place, e.g. the factory location where something is manufactured.</rdfs:comment>
    <rdfs:label>occurs at location</rdfs:label>
  </rdf:Description>
  <rdf:Description rdf:about="http://purl.org/dc/terms/title">
    <rdf:type rdf:resource="http://www.w3.org/2002/07/owl#AnnotationProperty"/>
  </rdf:Description>
  <rdf:Description rdf:about="http://w3id.org/CEON/ontology/processODP/hasExecutionInput">
    <rdf:type rdf:resource="http://www.w3.org/2002/07/owl#ObjectProperty"/>
    <rdfs:domain rdf:resource="http://w3id.org/CEON/ontology/processODP/ProcessExecution"/>
    <rdfs:comment>The situation before the execution takes place, i.e. the state of affairs before the process takes places, such as the set of components before they are assembled into a product object.</rdfs:comment>
    <rdfs:label>has execution input</rdfs:label>
  </rdf:Description>
  <rdf:Description rdf:about="http://purl.org/dc/terms/description">
    <rdf:type rdf:resource="http://www.w3.org/2002/07/owl#AnnotationProperty"/>
  </rdf:Description>
  <rdf:Description rdf:about="http://w3id.org/CEON/ontology/processODP/hasExecutionOutput">
    <rdf:type rdf:resource="http://www.w3.org/2002/07/owl#ObjectProperty"/>
    <rdfs:domain rdf:resource="http://w3id.org/CEON/ontology/processODP/ProcessExecution"/>
    <rdfs:comment>The situation after the execution takes place, i.e. the state of affairs before the process takes places, such as the assembled product object.</rdfs:comment>
    <rdfs:label>has execution output</rdfs:label>
  </rdf:Description>
  <rdf:Description rdf:about="http://w3id.org/CEON/ontology/processODP/">
    <rdf:type rdf:resource="http://www.w3.org/2002/07/owl#Ontology"/>
    <owl:versionIRI rdf:resource="http://w3id.org/CEON/ontology/processODP/0.3/"/>
    <dcterms:contributor>Eva Blomqvist</dcterms:contributor>
    <dcterms:contributor>Mikael Lindecrantz</dcterms:contributor>
    <dcterms:contributor>Robin Keskisärkkä</dcterms:contributor>
    <dcterms:created>2024-11-13</dcterms:created>
    <dcterms:creator>Huanyu Li</dcterms:creator>
    <dcterms:description>A core ODP of the CEON ontology network, defining aspects of the process concept.</dcterms:description>
    <dcterms:license>https://creativecommons.org/licenses/by/4.0/</dcterms:license>
    <dcterms:title>Circular Economy Ontology Network (CEON) - Process ODP</dcterms:title>
    <vann:preferredNamespacePrefix>processODP</vann:preferredNamespacePrefix>
    <vann:preferredNamespaceUri>http://w3id.org/CEON/ontology/processODP/</vann:preferredNamespaceUri>
    <odp:coversRequirements>Covers the following requirements from Onto-DESIDE D3.1: CVN-Process-3,4,5, C3-1, C4-2, C4-5, C4-7, C4-9, C13-2, E2-6</odp:coversRequirements>
    <rdfs:comment>A core ODP of the CEON ontology network, defining aspects of the process concept.</rdfs:comment>
    <rdfs:seeAlso rdf:resource="https://github.com/LiUSemWeb/CEON"/>
    <owl:versionInfo rdf:datatype="http://www.w3.org/2001/XMLSchema#decimal">0.3</owl:versionInfo>
  </rdf:Description>
  <rdf:Description rdf:nodeID="n45222b39aba54140964bb20f04669c55b1">
    <rdf:type rdf:resource="http://www.w3.org/2002/07/owl#Restriction"/>
    <owl:onProperty rdf:resource="http://w3id.org/CEON/ontology/processODP/hasProcessExecution"/>
    <owl:someValuesFrom rdf:resource="http://w3id.org/CEON/ontology/processODP/ProcessExecution"/>
  </rdf:Description>
  <rdf:Description rdf:about="http://w3id.org/CEON/ontology/processODP/hasProcessType">
    <rdf:type rdf:resource="http://www.w3.org/2002/07/owl#ObjectProperty"/>
    <rdfs:domain rdf:resource="http://w3id.org/CEON/ontology/processODP/Process"/>
    <rdfs:range rdf:resource="http://w3id.org/CEON/ontology/processODP/ProcessType"/>
    <rdfs:comment>The type of the process.</rdfs:comment>
    <rdfs:label>has process type</rdfs:label>
  </rdf:Description>
  <rdf:Description rdf:about="http://w3id.org/CEON/ontology/processODP/Transformation">
    <rdf:type rdf:resource="http://www.w3.org/2002/07/owl#Class"/>
    <rdfs:subClassOf rdf:resource="http://w3id.org/CEON/ontology/processODP/Process"/>
    <rdfs:subClassOf rdf:nodeID="n45222b39aba54140964bb20f04669c55b5"/>
    <rdfs:comment>A process that transforms some situation into another situation, i.e. changes the state of affairs of some actor, resource etc.</rdfs:comment>
    <rdfs:label>Transformation</rdfs:label>
  </rdf:Description>
  <rdf:Description rdf:about="http://w3id.org/CEON/ontology/processODP/hasProcessExecution">
    <rdf:type rdf:resource="http://www.w3.org/2002/07/owl#ObjectProperty"/>
    <rdfs:domain rdf:resource="http://w3id.org/CEON/ontology/processODP/Process"/>
    <rdfs:range rdf:resource="http://w3id.org/CEON/ontology/processODP/ProcessExecution"/>
    <rdfs:comment xml:lang="en">A process can have specific executions.</rdfs:comment>
    <rdfs:label xml:lang="en">has process execution</rdfs:label>
  </rdf:Description>
  <rdf:Description rdf:about="http://w3id.org/CEON/ontology/processODP/nextProcess">
    <rdf:type rdf:resource="http://www.w3.org/2002/07/owl#ObjectProperty"/>
    <rdfs:domain rdf:resource="http://w3id.org/CEON/ontology/processODP/Process"/>
    <rdfs:range rdf:resource="http://w3id.org/CEON/ontology/processODP/Process"/>
    <rdfs:comment>A relation between one process and the next one following it in some sequence of processes, e.g. a sequence of transformations in a material flow.</rdfs:comment>
    <rdfs:label>next process</rdfs:label>
  </rdf:Description>
  <rdf:Description rdf:about="http://w3id.org/CEON/ontology/processODP/occursAtTime">
    <rdf:type rdf:resource="http://www.w3.org/2002/07/owl#DatatypeProperty"/>
    <rdfs:domain rdf:resource="http://w3id.org/CEON/ontology/processODP/ProcessExecution"/>
    <rdfs:range rdf:resource="http://www.w3.org/2001/XMLSchema#dateTime"/>
    <rdfs:comment>Represents the time at which something takes place.</rdfs:comment>
    <rdfs:label>occurs at time</rdfs:label>
  </rdf:Description>
  <rdf:Description rdf:about="http://w3id.org/CEON/ontology/processODP/intialSituation">
    <rdf:type rdf:resource="http://www.w3.org/2002/07/owl#ObjectProperty"/>
    <rdfs:domain rdf:resource="http://w3id.org/CEON/ontology/processODP/ProcessExecution"/>
    <rdfs:range rdf:resource="http://w3id.org/CEON/ontology/processODP/Situation"/>
    <rdfs:comment>The situation before executing a process.</rdfs:comment>
    <rdfs:label>initial situation</rdfs:label>
  </rdf:Description>
  <rdf:Description rdf:about="http://w3id.org/CEON/ontology/processODP/Process">
    <rdf:type rdf:resource="http://www.w3.org/2002/07/owl#Class"/>
    <rdfs:subClassOf rdf:nodeID="n45222b39aba54140964bb20f04669c55b1"/>
    <rdfs:comment xml:lang="en">Set of interrelated or interacting activities that transforms inputs into outputs.</rdfs:comment>
    <rdfs:isDefinedBy>ISO 59004:2024  - 3.5.5 process</rdfs:isDefinedBy>
    <rdfs:label>Process</rdfs:label>
  </rdf:Description>
  <rdf:Description rdf:about="http://w3id.org/CEON/ontology/processODP/hasOutput">
    <rdf:type rdf:resource="http://www.w3.org/2002/07/owl#ObjectProperty"/>
    <rdfs:domain rdf:resource="http://w3id.org/CEON/ontology/processODP/Process"/>
    <rdfs:comment>The output situation of after the process is executed, i.e. the state of affairs after the process is executed.</rdfs:comment>
    <rdfs:label>has output</rdfs:label>
  </rdf:Description>
  <rdf:Description rdf:about="http://w3id.org/CEON/ontology/processODP/ProcessExecution">
    <rdf:type rdf:resource="http://www.w3.org/2002/07/owl#Class"/>
    <rdfs:subClassOf rdf:nodeID="n45222b39aba54140964bb20f04669c55b2"/>
    <rdfs:subClassOf rdf:nodeID="n45222b39aba54140964bb20f04669c55b3"/>
    <rdfs:comment>An execution of a specific process at a specific location and time point.</rdfs:comment>
    <rdfs:label>Process execution</rdfs:label>
  </rdf:Description>
  <rdf:Description rdf:about="http://w3id.org/CEON/ontology/processODP/resultingSituation">
    <rdf:type rdf:resource="http://www.w3.org/2002/07/owl#ObjectProperty"/>
    <rdfs:domain rdf:resource="http://w3id.org/CEON/ontology/processODP/ProcessExecution"/>
    <rdfs:range rdf:resource="http://w3id.org/CEON/ontology/processODP/Situation"/>
    <rdfs:comment>The situation after the execution of a process.</rdfs:comment>
    <rdfs:label>resulting situation</rdfs:label>
  </rdf:Description>
  <rdf:Description rdf:about="http://w3id.org/CEON/ontology/processODP/nextExecution">
    <rdf:type rdf:resource="http://www.w3.org/2002/07/owl#ObjectProperty"/>
    <rdfs:domain rdf:resource="http://w3id.org/CEON/ontology/processODP/ProcessExecution"/>
    <rdfs:range rdf:resource="http://w3id.org/CEON/ontology/processODP/ProcessExecution"/>
    <rdfs:comment>A relation between one execution and the next one following it in some sequence of executions, e.g. a sequence of transformations in a material flow.</rdfs:comment>
    <rdfs:label>next execution</rdfs:label>
  </rdf:Description>
  <rdf:Description rdf:nodeID="n45222b39aba54140964bb20f04669c55b2">
    <rdf:type rdf:resource="http://www.w3.org/2002/07/owl#Restriction"/>
    <owl:onProperty rdf:resource="http://w3id.org/CEON/ontology/processODP/hasExecutionInput"/>
    <owl:someValuesFrom rdf:resource="http://www.w3.org/2002/07/owl#Thing"/>
  </rdf:Description>
  <rdf:Description rdf:about="http://w3id.org/CEON/ontology/processODP/hasInput">
    <rdf:type rdf:resource="http://www.w3.org/2002/07/owl#ObjectProperty"/>
    <rdfs:domain rdf:resource="http://w3id.org/CEON/ontology/processODP/Process"/>
    <rdfs:comment>The situation before the process has an execution, i.e. the state of affairs before the process takes places, such as the set of components before they are assembled into a product.</rdfs:comment>
    <rdfs:label>has input</rdfs:label>
  </rdf:Description>
  <rdf:Description rdf:nodeID="n45222b39aba54140964bb20f04669c55b3">
    <rdf:type rdf:resource="http://www.w3.org/2002/07/owl#Restriction"/>
    <owl:onProperty rdf:resource="http://w3id.org/CEON/ontology/processODP/hasExecutionOutput"/>
    <owl:someValuesFrom rdf:resource="http://www.w3.org/2002/07/owl#Thing"/>
  </rdf:Description>
  <rdf:Description rdf:nodeID="n45222b39aba54140964bb20f04669c55b5">
    <rdf:type rdf:resource="http://www.w3.org/2002/07/owl#Restriction"/>
    <owl:onProperty rdf:resource="http://w3id.org/CEON/ontology/processODP/hasTransformationExecution"/>
    <owl:someValuesFrom rdf:resource="http://w3id.org/CEON/ontology/processODP/TransformationExecution"/>
  </rdf:Description>
  <rdf:Description rdf:about="http://purl.org/vocab/vann/preferredNamespaceUri">
    <rdf:type rdf:resource="http://www.w3.org/2002/07/owl#AnnotationProperty"/>
  </rdf:Description>
  <rdf:Description rdf:about="http://w3id.org/CEON/ontology/processODP/hasPart">
    <rdf:type rdf:resource="http://www.w3.org/2002/07/owl#ObjectProperty"/>
    <rdf:type rdf:resource="http://www.w3.org/2002/07/owl#TransitiveProperty"/>
    <rdfs:domain rdf:resource="http://w3id.org/CEON/ontology/processODP/Process"/>
    <rdfs:range rdf:resource="http://w3id.org/CEON/ontology/processODP/Process"/>
    <rdfs:comment>A process can consists of several part, which are sub-processes.</rdfs:comment>
    <rdfs:label>has part</rdfs:label>
  </rdf:Description>
  <rdf:Description rdf:about="http://w3id.org/CEON/ontology/processODP/isSettingFor">
    <rdf:type rdf:resource="http://www.w3.org/2002/07/owl#ObjectProperty"/>
    <rdfs:domain rdf:resource="http://w3id.org/CEON/ontology/processODP/Situation"/>
    <rdfs:comment>The thing(s) that this situation is the setting for, e.g. a resource that is in a certain state.</rdfs:comment>
    <rdfs:label>is the setting for</rdfs:label>
  </rdf:Description>
  <rdf:Description rdf:about="http://w3id.org/CEON/ontology/processODP/ProcessType">
    <rdf:type rdf:resource="http://www.w3.org/2002/07/owl#Class"/>
    <rdfs:comment>The type of a process.</rdfs:comment>
    <rdfs:label>Process type</rdfs:label>
  </rdf:Description>
  <rdf:Description rdf:about="http://purl.org/dc/terms/creator">
    <rdf:type rdf:resource="http://www.w3.org/2002/07/owl#AnnotationProperty"/>
  </rdf:Description>
  <rdf:Description rdf:about="http://purl.org/vocab/vann/preferredNamespacePrefix">
    <rdf:type rdf:resource="http://www.w3.org/2002/07/owl#AnnotationProperty"/>
  </rdf:Description>
  <rdf:Description rdf:about="http://w3id.org/CEON/ontology/location/Location">
    <rdf:type rdf:resource="http://www.w3.org/2002/07/owl#Class"/>
  </rdf:Description>
  <rdf:Description rdf:nodeID="n45222b39aba54140964bb20f04669c55b4">
    <rdf:type rdf:resource="http://www.w3.org/2002/07/owl#Restriction"/>
    <owl:onProperty rdf:resource="http://w3id.org/CEON/ontology/processODP/isSettingFor"/>
    <owl:someValuesFrom rdf:resource="http://www.w3.org/2002/07/owl#Thing"/>
  </rdf:Description>
  <rdf:Description rdf:about="http://purl.org/dc/terms/created">
    <rdf:type rdf:resource="http://www.w3.org/2002/07/owl#AnnotationProperty"/>
  </rdf:Description>
  <rdf:Description rdf:about="http://www.ontologydesignpatterns.org/schemas/cpannotationschema.owl#coversRequirements">
    <rdf:type rdf:resource="http://www.w3.org/2002/07/owl#AnnotationProperty"/>
  </rdf:Description>
  <rdf:Description rdf:about="http://w3id.org/CEON/ontology/processODP/Situation">
    <rdf:type rdf:resource="http://www.w3.org/2002/07/owl#Class"/>
    <rdfs:subClassOf rdf:nodeID="n45222b39aba54140964bb20f04669c55b4"/>
    <rdfs:comment>A situation that may involve some resources and actors, i.e. a state of affairs at a certain point in time.</rdfs:comment>
    <rdfs:label>Situation</rdfs:label>
  </rdf:Description>
  <rdf:Description rdf:about="http://purl.org/dc/terms/license">
    <rdf:type rdf:resource="http://www.w3.org/2002/07/owl#AnnotationProperty"/>
  </rdf:Description>
  <rdf:Description rdf:about="http://purl.org/dc/terms/contributor">
    <rdf:type rdf:resource="http://www.w3.org/2002/07/owl#AnnotationProperty"/>
  </rdf:Description>
</rdf:RDF>
