@prefix : <http://w3id.org/CEON/ontology/provenance/> .
@prefix owl: <http://www.w3.org/2002/07/owl#> .
@prefix rdf: <http://www.w3.org/1999/02/22-rdf-syntax-ns#> .
@prefix xml: <http://www.w3.org/XML/1998/namespace> .
@prefix xsd: <http://www.w3.org/2001/XMLSchema#> .
@prefix rdfs: <http://www.w3.org/2000/01/rdf-schema#> .
@prefix vann: <http://purl.org/vocab/vann/> .
@prefix dcterms: <http://purl.org/dc/terms/> .
@prefix resourceODP: <http://w3id.org/CEON/ontology/resourceODP/> .
@base <http://w3id.org/CEON/ontology/provenance/> .

<http://w3id.org/CEON/ontology/provenance/> rdf:type owl:Ontology ;
                                             owl:versionIRI <http://w3id.org/CEON/ontology/provenance/0.1/> ;
                                             owl:imports <http://w3id.org/CEON/ontology/resourceODP/0.2/> ,
                                                         <http://www.w3.org/ns/prov-o-20130430> ;
                                             dcterms:contributor "Huanyu Li" ,
                                                                 "Mikael Lindecrantz" ,
                                                                 "Robin Keskisärkkä" ;
                                             dcterms:created "2023-09-18" ;
                                             dcterms:creator "Eva Blomqvist" ;
                                             dcterms:description "A specialisation of PROV-O for expressing provenance of CEON resources." ;
                                             dcterms:license "https://creativecommons.org/licenses/by/4.0/"^^xsd:string ;
                                             dcterms:title "Circular Economy Ontology Network (CEON) - Provenance" ;
                                             vann:preferredNamespacePrefix "CEONprov" ;
                                             vann:preferredNamespaceUri "http://w3id.org/CEON/ontology/provenance/" ;
                                             owl:versionInfo "0.1" .

#################################################################
#    Classes
#################################################################

###  http://w3id.org/CEON/ontology/provenance/Statement
:Statement rdf:type owl:Class ;
           rdfs:subClassOf <http://www.w3.org/ns/prov#Entity> ;
           rdfs:comment "Generic class representing the concept of a statement, i.e. some piece of information, fact etc that is expressed in the data. Effectively used to reify relations (triples) in the data, and express information about them." ;
           rdfs:label "statement" .


###  http://w3id.org/CEON/ontology/resourceODP/Resource
resourceODP:Resource rdfs:subClassOf <http://www.w3.org/ns/prov#Entity> .

#################################################################
#    Object Properties
#################################################################

###  http://w3id.org/CEON/ontology/provenance/statementAbout
:statementAbout rdf:type owl:ObjectProperty ;
           rdfs:domain :Statement ;
           rdfs:comment "Generic property to express what the statement is about, i.e. what is involved in the statement." ;
           rdfs:label "statement about" .

#################################################################
#    Data properties
#################################################################

###  http://w3id.org/CEON/ontology/provenance/statementValue
:statementValue rdf:type owl:DatatypeProperty ;
          rdfs:domain :Statement ;
           rdfs:comment "Generic property to express values, e.g. literals, that are involved in this statement." ;
           rdfs:label "statement value" .


###  Generated by the OWL API (version 4.5.9.2019-02-01T07:24:44Z) https://github.com/owlcs/owlapi
