@prefix : <http://w3id.org/CEON/ontology/value/> .
@prefix actorODP: <http://w3id.org/CEON/ontology/actorODP/> .
@prefix dcterms: <http://purl.org/dc/terms/> .
@prefix odp: <http://www.ontologydesignpatterns.org/schemas/cpannotationschema.owl#> .
@prefix owl: <http://www.w3.org/2002/07/owl#> .
@prefix rdf: <http://www.w3.org/1999/02/22-rdf-syntax-ns#> .
@prefix rdfs: <http://www.w3.org/2000/01/rdf-schema#> .
@prefix vann: <http://purl.org/vocab/vann/> .
@prefix xsd: <http://www.w3.org/2001/XMLSchema#> .

: a owl:Ontology ;
    dcterms:contributor "Eva Blomqvist",
        "Mikael Lindecrantz",
        "Robin Keskisärkkä" ;
    dcterms:created "2025-05-20"^^xsd:date ;
    dcterms:creator "Huanyu Li" ;
    dcterms:description "A core ODP of the CEON ontology network, defining aspects of the value concept." ;
    dcterms:issued "2025-06-30"^^xsd:date ;
    dcterms:license "https://creativecommons.org/licenses/by/4.0/" ;
    dcterms:publisher "Onto-DESIDE" ;
    dcterms:title "Circular Economy Ontology Network (CEON) - Value Module" ;
    vann:preferredNamespacePrefix "ceon-value" ;
    vann:preferredNamespaceUri "https://w3id.org/CEON/ontoloy/value/" ;
    odp:coversRequirements "Covers the following requirements from Onto-DESIDE D3.2: CE1-3, CE5-16, CE5-17, CE5-19, CE7-8, CE9-4, CE10-10, CE11-2, C2-1, C4-4, C4-6, C5-2." ;
    rdfs:comment "A core ODP of the CEON ontology network, defining aspects of the value concept." ;
    rdfs:seeAlso <https://github.com/LiUSemWeb/CEON> ;
    owl:imports <http://w3id.org/CEON/ontology/actorODP/0.4/> ;
    owl:versionIRI <http://w3id.org/CEON/ontology/value/0.3/> ;
    owl:versionInfo 0.3 .

:EconomicValue a owl:Class ;
    rdfs:label "Economic Value" ;
    rdfs:comment "Use/Economics value represents how a thing (e.g., a product or service) match some goals or needs of an actor under some circumstances." ;
    rdfs:subClassOf :Value ;
    owl:equivalentClass :UseValue .

:EnvironmentalValue a owl:Class ;
    rdfs:label "Environmental Value" ;
    rdfs:comment "Environmental value represents how a thing (e.g., a product or service) match some environmental goals or needs of an actor under some circumstances." ;
    rdfs:subClassOf :Value .

:ExchangeValue a owl:Class ;
    rdfs:label "Exchange Value" ;
    rdfs:comment "Exchange value represents the worth of a product, resource, service in a exchange setting, i.e., a product, resource, service is traded or sold." ;
    rdfs:subClassOf :Value .

:SocialValue a owl:Class ;
    rdfs:label "Social Value" ;
    rdfs:comment "Social value represents how a thing (e.g., a product or service) match some social goals or needs of an actor under some circumstances." ;
    rdfs:subClassOf :Value .

:ValueConsumer a :ValueParticipationRole,
        owl:NamedIndividual .

:ValueContributor a :ValueParticipationRole,
        owl:NamedIndividual .

:ValueCreator a :ValueParticipationRole,
        owl:NamedIndividual .

:ValueDestroyer a :ValueParticipationRole,
        owl:NamedIndividual .

:ValueDistributor a :ValueParticipationRole,
        owl:NamedIndividual .

:ValueEvaluator a :ValueParticipationRole,
        owl:NamedIndividual .

:hasPerception a owl:ObjectProperty ;
    rdfs:label "has perception" ;
    rdfs:comment "An actor perceive specific values, or a value proposition is about specific values." ;
    rdfs:domain [ a owl:Class ;
            owl:unionOf ( actorODP:Actor :ValueProposition ) ] ;
    rdfs:range :ValuePerception .

:hasValuableResource a owl:ObjectProperty ;
    rdfs:label "has valuable resource" ;
    rdfs:comment "A value participation has participating resources." ;
    rdfs:domain :ValueParticipation ;
    rdfs:range <http://w3id.org/CEON/ontology/resourceODP/Resource> ;
    rdfs:subPropertyOf owl:topObjectProperty .

:hasValueParticipantRole a owl:ObjectProperty ;
    rdfs:label "has value participant role" ;
    rdfs:comment "Holds the value of the role of the value participant in this value participation relation." ;
    rdfs:domain :ValueParticipation ;
    rdfs:range :ValueParticipationRole ;
    rdfs:subPropertyOf actorODP:participantRole .

:onValueParticipation a owl:ObjectProperty ;
    rdfs:label "on value participation" ;
    rdfs:comment "A perception is on specific value participations." ;
    rdfs:domain :ValuePerception ;
    rdfs:range :ValueParticipation .

:proposedBy a owl:ObjectProperty ;
    rdfs:label "proposed by" ;
    rdfs:comment "A value proposition is proposed by specific actors." ;
    rdfs:domain :ValueProposition ;
    rdfs:range actorODP:Actor .

:targettingResource a owl:ObjectProperty ;
    rdfs:label "targetting resource" ;
    rdfs:comment "A value proposition is about some resources." ;
    rdfs:domain :ValueProposition ;
    rdfs:range <http://w3id.org/CEON/ontology/resourceODP/Resource> ;
    rdfs:subPropertyOf :hasVPTargets .

xsd:date a rdfs:Datatype .

xsd:gMonthYear a rdfs:Datatype .

xsd:gYear a rdfs:Datatype .

:UseValue a owl:Class ;
    rdfs:label "Use Value" ;
    rdfs:comment "Use/Economics value represents how a thing (e.g., a product or service) match some goals or needs of an actor under some circumstances." ;
    rdfs:subClassOf :Value .

:hasAimedValue a owl:ObjectProperty ;
    rdfs:label "has aimed value" ;
    rdfs:comment "A value proposition has specific aimed values." ;
    rdfs:domain :ValueProposition ;
    rdfs:range :Value .

:hasAssociatedValue a owl:ObjectProperty ;
    rdfs:label "has associated value" ;
    rdfs:comment "A value perception about creating/destoring/missing some value." ;
    rdfs:domain :ValuePerception ;
    rdfs:range :Value ;
    rdfs:subPropertyOf owl:topObjectProperty .

:targettingActor a owl:ObjectProperty ;
    rdfs:label "targetting actor" ;
    rdfs:comment "A value proposition is about some actors." ;
    rdfs:domain :ValueProposition ;
    rdfs:range actorODP:Actor ;
    rdfs:subPropertyOf :hasVPTargets .

:targettingValueParticipation a owl:ObjectProperty ;
    rdfs:label "targetting value participation" ;
    rdfs:comment "A value proposition is about some participation." ;
    rdfs:domain :ValueProposition ;
    rdfs:range :ValueParticipation ;
    rdfs:subPropertyOf :hasVPTargets .

<http://w3id.org/CEON/ontology/resourceODP/Resource> a owl:Class .

:ValuePerception a owl:Class ;
    rdfs:label "Value Perception" ;
    rdfs:comment "Value perception of an actor determines specifc values." .

:hasVPTargets a owl:ObjectProperty ;
    rdfs:label "has value proposition targets" ;
    rdfs:comment "A value proposition is proposed about specific actors, participations or resources." .

:ValueParticipation a owl:Class ;
    rdfs:label "Value Participation" ;
    rdfs:comment "A participation that may create/destory/miss value." ;
    rdfs:subClassOf [ a owl:Restriction ;
            owl:onProperty :hasAssociatedValue ;
            owl:someValuesFrom :Value ],
        actorODP:Participation .

:ValueProposition a owl:Class ;
    rdfs:label "Value Proposition" ;
    rdfs:comment "Proposed or intended value outcome of some process, action or collaboration." ;
    rdfs:subClassOf [ a owl:Restriction ;
            owl:onProperty :hasAimedValue ;
            owl:someValuesFrom :Value ],
        [ a owl:Restriction ;
            owl:onProperty :targettingActor ;
            owl:someValuesFrom actorODP:Actor ],
        [ a owl:Restriction ;
            owl:onProperty :targettingValueParticipation ;
            owl:someValuesFrom :ValueParticipation ] .

:ValueParticipationRole a owl:Class ;
    rdfs:label "Value Participation Role" ;
    rdfs:comment "A role that a value participant can take." ;
    rdfs:subClassOf actorODP:Role .

:Value a owl:Class ;
    rdfs:label "Value" ;
    rdfs:comment "Gain(s) or benefit(s) from satisfying needs and expectations,	in relation to the use	and conservation of resources. EXAMPLE: Revenue, savings, productivity, sustainability, satisfaction, empowerment, engagement, experience, public health, trust. Value is relative to, and determined by the perception of, those interested party(ies) able to capture it. Value can be financial or non-financial, e.g. social, environmental, other gains or benefits. Value is dynamic over time."@en ;
    rdfs:isDefinedBy "ISO 59004:2024 - 3.1.7 value" .

