@prefix : <http://w3id.org/CEON/ontology/material/> .
@prefix dcterms: <http://purl.org/dc/terms/> .
@prefix odp: <http://www.ontologydesignpatterns.org/schemas/cpannotationschema.owl#> .
@prefix owl: <http://www.w3.org/2002/07/owl#> .
@prefix rdfs: <http://www.w3.org/2000/01/rdf-schema#> .
@prefix resourceODP: <http://w3id.org/CEON/ontology/resourceODP/> .
@prefix vann: <http://purl.org/vocab/vann/> .
@prefix xsd: <http://www.w3.org/2001/XMLSchema#> .

: a owl:Ontology ;
    dcterms:contributor "Eva Blomqvist",
        "Mikael Lindecrantz",
        "Robin Keskisärkkä" ;
    dcterms:created "2025-03-20"^^xsd:date ;
    dcterms:creator "Huanyu Li" ;
    dcterms:description "The Material module of CEON (Circular Economy Ontology Network)." ;
    dcterms:issued "2025-06-30"^^xsd:date ;
    dcterms:license "https://creativecommons.org/licenses/by/4.0/" ;
    dcterms:publisher "Onto-DESIDE" ;
    dcterms:title "Circular Economy Ontology Network (CEON) - Material Module" ;
    vann:preferredNamespacePrefix "ceon-material" ;
    vann:preferredNamespaceUri "http://w3id.org/CEON/ontology/material/" ;
    odp:coversRequirements "In addition to requirements covered by imported ODPs, covers the following requirements from Onto-DESIDE D3.1: CVN-Resource-2, CVN-ResourceType-4, C3-3, E1-3, E2-4, E5-2, T1-1, T10-2.",
        "In addition to requirements covered by imported ODPs, covers the following requirements from Onto-DESIDE D3.2: CE5-2, C3-3, E1-3, E2-4, E5-2, T1-1, T10-2." ;
    rdfs:seeAlso <https://github.com/LiUSemWeb/CEON> ;
    owl:imports <http://w3id.org/CEON/ontology/resourceODP/0.5/> ;
    owl:priorVersion 0.3 ;
    owl:versionIRI <http://w3id.org/CEON/ontology/material/0.4/> ;
    owl:versionInfo 0.4 .

:Aluminum a owl:Class ;
    rdfs:label "Aluminum" ;
    rdfs:comment "Aluminum is a chemical element with the symbol Al and atomic number 13." ;
    rdfs:subClassOf :ChemicalElement .

:Boron a owl:Class ;
    rdfs:label "Boron" ;
    rdfs:comment "Boron is a chemical element with the symbol B and atomic number 5." ;
    rdfs:subClassOf :ChemicalElement .

:Cellulose a owl:Class ;
    rdfs:label "Cellulose" ;
    rdfs:comment "Cellulose is an organic compound with chemical formula (C6H10O5)n." ;
    rdfs:subClassOf :Material .

:Cerium a owl:Class ;
    rdfs:label "Cerium" ;
    rdfs:comment "Cerium is a chemical element with the symbol Ce and atomic number 58." ;
    rdfs:subClassOf :RareEarthElement .

:Chromium a owl:Class ;
    rdfs:label "Chromium" ;
    rdfs:comment "Chromium is a chemical element with the symbol Cr and atomic number 24." ;
    rdfs:subClassOf :ChemicalElement .

:Copper a owl:Class ;
    rdfs:label "Copper" ;
    rdfs:comment "Copper is a chemical element with the symbol Cu and atomic number 29." ;
    rdfs:subClassOf :ChemicalElement .

:Dysprosium a owl:Class ;
    rdfs:label "Dysorisium" ;
    rdfs:comment "Dysprosium is a chemical element with the symbol Dy and atomic number 66." ;
    rdfs:subClassOf :RareEarthElement .

:Erbium a owl:Class ;
    rdfs:label "Erbium" ;
    rdfs:comment "Erbium is a chemical element with the symbol Er and atomic number 68." ;
    rdfs:subClassOf :RareEarthElement .

:Europium a owl:Class ;
    rdfs:label "Europium" ;
    rdfs:comment "Europium is a chemical element with the symbol Eu and atomic number 63." ;
    rdfs:subClassOf :RareEarthElement .

:Gadolinium a owl:Class ;
    rdfs:label "Gadolinium" ;
    rdfs:comment "Gadolinium is a chemical element with the symbol Gd and atomic number 64." ;
    rdfs:subClassOf :RareEarthElement .

:Holmium a owl:Class ;
    rdfs:label "Holmium" ;
    rdfs:comment "Holmium is a chemical element with the symbol Ho and atomic number 67." ;
    rdfs:subClassOf :RareEarthElement .

:Iron a owl:Class ;
    rdfs:label "Iron" ;
    rdfs:comment "Iron is a chemical element with the symbol Fe and atomic number 26." ;
    rdfs:subClassOf :ChemicalElement .

:Lanthanum a owl:Class ;
    rdfs:label "Lanthanum" ;
    rdfs:comment "Lanthanum is a chemical element with the symbol Lal and atomic number 57." ;
    rdfs:subClassOf :RareEarthElement .

:Lutetium a owl:Class ;
    rdfs:label "Lutetium" ;
    rdfs:comment "Lutetium is a chemical element with the symbol Lu and atomic number 71." ;
    rdfs:subClassOf :RareEarthElement .

:Magnesium a owl:Class ;
    rdfs:label "Magnesium" ;
    rdfs:comment "Magnesium is a chemical element with the symbol Mg and atomic number 12." ;
    rdfs:subClassOf :ChemicalElement .

:Manganese a owl:Class ;
    rdfs:label "Manganese" ;
    rdfs:comment "Manganese is a chemical element with the symbol Mn and atomic number 25." ;
    rdfs:subClassOf :ChemicalElement .

:MolecularEntity a owl:Class ;
    rdfs:label "Molecular Entity" ;
    rdfs:comment "A molecular entity means a singular/distinguishable entity. It can be for instance, atom, ion." ;
    rdfs:seeAlso "http://emmo.info/emmo#EMMO_21205421_5783_4d3e_81e5_10c5d894a88a",
        "http://purl.obolibrary.org/obo/chebi#23367" ;
    rdfs:subClassOf :ChemicalEntity .

:Neodymium a owl:Class ;
    rdfs:label "Neodymium" ;
    rdfs:comment "Neodymium is a chemical element with the symbol Nd and atomic number 60." ;
    rdfs:subClassOf :RareEarthElement .

:Nickel a owl:Class ;
    rdfs:label "Nickel" ;
    rdfs:comment "Nickel is a chemical element with the symbol Ni and atomic number 28." ;
    rdfs:subClassOf :ChemicalElement .

:Niobium a owl:Class ;
    rdfs:label "Niobium" ;
    rdfs:comment "Niobium is a chemical element with the symbol Nb and atomic number 41." ;
    rdfs:subClassOf :ChemicalElement .

:Praseodymium a owl:Class ;
    rdfs:label "Praseodymium" ;
    rdfs:comment "Praseodymium is a chemical element with the symbol Pr and atomic number 59." ;
    rdfs:subClassOf :RareEarthElement .

:Promethium a owl:Class ;
    rdfs:label "Promethium" ;
    rdfs:comment "Promethium is a chemical element with the symbol Pm and atomic number 61." ;
    rdfs:subClassOf :RareEarthElement .

:Samarium a owl:Class ;
    rdfs:label "Samarium" ;
    rdfs:comment "Samarium is a chemical element with the symbol Sm and atomic number 62." ;
    rdfs:subClassOf :RareEarthElement .

:Scandium a owl:Class ;
    rdfs:label "Scandium" ;
    rdfs:comment "Scandium is a chemical element with the symbol Sc and atomic number 21." ;
    rdfs:subClassOf :RareEarthElement .

:Silicon a owl:Class ;
    rdfs:label "Silicon" ;
    rdfs:comment "Silicon is a chemical element with the symbol Si and atomic number 14." ;
    rdfs:subClassOf :ChemicalElement .

:Tantalum a owl:Class ;
    rdfs:label "Tantalum" ;
    rdfs:comment "Tantalum is a chemical element with the symbol Ta and atomic number 73." ;
    rdfs:subClassOf :RareEarthElement .

:Terbium a owl:Class ;
    rdfs:label "Terbium" ;
    rdfs:comment "Terbium is a chemical element with the symbol Tb and atomic number 65." ;
    rdfs:subClassOf :RareEarthElement .

:Thulium a owl:Class ;
    rdfs:label "Thulium" ;
    rdfs:comment "Thulium is a chemical element with the symbol Tm and atomic number 69." ;
    rdfs:subClassOf :RareEarthElement .

:Titanium a owl:Class ;
    rdfs:label "Titanium" ;
    rdfs:comment "Titanium is a chemical element with the symbol Ti and atomic number 22." ;
    rdfs:subClassOf :ChemicalElement .

:Ytterbium a owl:Class ;
    rdfs:label "Ytterbium" ;
    rdfs:comment "Yteerbium is a chemical element with the symbol Yb and atomic number 70." ;
    rdfs:subClassOf :RareEarthElement .

:Yttrium a owl:Class ;
    rdfs:label "Yttrium" ;
    rdfs:comment "Yttrium is a chemical element with the symbol Y and atomic number 39." ;
    rdfs:subClassOf :RareEarthElement .

:Zinc a owl:Class ;
    rdfs:label "Zinc" ;
    rdfs:comment "Zinc is a chemical element with the symbol Zn and atomic number 30." ;
    rdfs:subClassOf :ChemicalElement .

:anonymousFormula a owl:DatatypeProperty ;
    rdfs:label "anonymous formula" ;
    rdfs:comment "anonymousFormula represents that a molecular entity has the anonymous formula in a string." ;
    rdfs:seeAlso "https://w3id.org/mdo/structure/AnonymousFormula" .

:descriptiveFormula a owl:DatatypeProperty ;
    rdfs:label "descriptive formula" ;
    rdfs:comment "descriptiveFormula represents that a molecular entity has the descriptive formula in a string." ;
    rdfs:seeAlso "https://w3id.org/mdo/structure/DescriptiveFormula" .

:hasMaterialComponent a owl:ObjectProperty ;
    rdfs:label "has material component" ;
    rdfs:comment "hasMaterialComponent intends to represent that a material can have a collection of components." ;
    rdfs:domain :Material ;
    rdfs:range :MaterialComponent .

:hillFormula a owl:DatatypeProperty ;
    rdfs:label "hill formula" ;
    rdfs:comment "hillFormula represents that a composition has the hill formula in a string." ;
    rdfs:seeAlso "https://w3id.org/mdo/structure/HillFormula" .

:reducedChemicalFormula a owl:DatatypeProperty ;
    rdfs:label "reduced chemical formula" ;
    rdfs:comment "reducedChemicalFormula represents that a molecular entity has the reduced chemical formula in a string." ;
    rdfs:seeAlso "https://w3id.org/mdo/structure/ReducedFormula" .

:ChemicalSubstance a owl:Class ;
    rdfs:label "Chemical Substance" ;
    rdfs:comment "A chemical substance is made up of a collection of molecular entities." ;
    rdfs:seeAlso "http://emmo.info/emmo#EMMO_df96cbb6_b5ee_4222_8eab_b3675df24bea",
        "http://purl.obolibrary.org/obo/chebi#59999" ;
    rdfs:subClassOf :ChemicalEntity .

:MaterialComponent a owl:Class ;
    rdfs:label "Material Component" ;
    rdfs:comment "A material component is a part of a material." ;
    rdfs:subClassOf resourceODP:Constituent .

:hasChemicalEntity a owl:ObjectProperty ;
    rdfs:label "has chemical entity" ;
    rdfs:comment "hasChemicalEntity intends to represent that a material can have a collection of chemical entities." ;
    rdfs:domain :Material ;
    rdfs:range :ChemicalEntity .

resourceODP:Constituent a owl:Class .

resourceODP:Matter a owl:Class .

:Material a owl:Class ;
    rdfs:label "Material" ;
    rdfs:comment "Material as a sub-concept of Matter, can be a substance or a collection of substance which a physical object is composed of." ;
    rdfs:seeAlso "http://emmo.info/emmo#EMMO_4207e895_8b83_4318_996a_72cfb32acd94",
        "https://w3id.org/mdo/core/Material" ;
    rdfs:subClassOf [ a owl:Restriction ;
            owl:onProperty :hasChemicalEntity ;
            owl:someValuesFrom :ChemicalEntity ],
        resourceODP:Matter .

:ChemicalEntity a owl:Class ;
    rdfs:label "Chemical Entity" ;
    rdfs:comment "A chemical entity is an abstraction of entities that can compose matter. For instance, a chemical entity can be a molecular entity or a chemical substance." ;
    rdfs:seeAlso "http://emmo.info/emmo#EMMO_47338839_6cca_4a8e_b565_3c4d5517e2c0",
        "http://purl.obolibrary.org/obo/chebi#24431" ;
    rdfs:subClassOf resourceODP:Matter .

:ChemicalElement a owl:Class ;
    rdfs:label "Chemical Element" ;
    rdfs:comment "A chemical element is a chemical substance whose atoms all have the same number of protons." ;
    rdfs:subClassOf :ChemicalSubstance .

:RareEarthElement a owl:Class ;
    rdfs:label "Rare Earth Element" ;
    rdfs:comment "Rare earth elements is a set of 17 nearly indistinguishable lustrous silvery-white soft heavy metals." ;
    rdfs:subClassOf :ChemicalElement .

