<?xml version="1.0" encoding="utf-8"?>
<rdf:RDF
   xmlns:owl="http://www.w3.org/2002/07/owl#"
   xmlns:rdf="http://www.w3.org/1999/02/22-rdf-syntax-ns#"
   xmlns:rdfs="http://www.w3.org/2000/01/rdf-schema#"
>
  <rdf:Description rdf:about="http://www.semanticweb.org/evabl45/ontologies/2023/8/untitled-ontology-86/isRealizationOf">
    <rdf:type rdf:resource="http://www.w3.org/2002/07/owl#ObjectProperty"/>
    <rdfs:domain rdf:nodeID="nfc0bec8256f84fce82d7a0bf9e82b550b1"/>
    <rdfs:range rdf:resource="http://w3id.org/CEON/ontology/resourceODP/Information"/>
    <rdfs:comment>The physical or digital realisation of a piece of information, e.g. a pdf file that stores the information about a product.</rdfs:comment>
    <rdfs:label>is realization of</rdfs:label>
  </rdf:Description>
  <rdf:Description rdf:about="http://www.semanticweb.org/evabl45/ontologies/2023/8/untitled-ontology-86/Statement">
    <rdf:type rdf:resource="http://www.w3.org/2002/07/owl#Class"/>
    <rdfs:subClassOf rdf:resource="http://w3id.org/CEON/ontology/resourceODP/Information"/>
    <rdfs:comment>A single fact, or statement about something. Usually contained within some larger piece of information, e.g. a document.</rdfs:comment>
    <rdfs:label>Statement</rdfs:label>
  </rdf:Description>
  <rdf:Description rdf:about="http://w3id.org/CEON/ontology/datasheet/">
    <rdf:type rdf:resource="http://www.w3.org/2002/07/owl#Ontology"/>
    <owl:versionIRI rdf:resource="http://w3id.org/CEON/ontology/datasheet/0.1/"/>
    <owl:imports rdf:resource="http://w3id.org/CEON/ontology/resourceODP/0.2/"/>
    <owl:imports rdf:resource="http://www.w3.org/ns/prov-o-20130430"/>
  </rdf:Description>
  <rdf:Description rdf:nodeID="nfc0bec8256f84fce82d7a0bf9e82b550b1">
    <rdf:type rdf:resource="http://www.w3.org/2002/07/owl#Class"/>
    <owl:unionOf rdf:nodeID="nfc0bec8256f84fce82d7a0bf9e82b550b2"/>
  </rdf:Description>
  <rdf:Description rdf:nodeID="nfc0bec8256f84fce82d7a0bf9e82b550b4">
    <rdf:type rdf:resource="http://www.w3.org/2002/07/owl#Restriction"/>
    <owl:onProperty rdf:resource="http://w3id.org/CEON/ontology/resourceODP/containsInformation"/>
    <owl:someValuesFrom rdf:resource="http://www.semanticweb.org/evabl45/ontologies/2023/8/untitled-ontology-86/Statement"/>
  </rdf:Description>
  <rdf:Description rdf:nodeID="nfc0bec8256f84fce82d7a0bf9e82b550b3">
    <rdf:first rdf:resource="http://w3id.org/CEON/ontology/resourceODP/PhysicalObject"/>
    <rdf:rest rdf:resource="http://www.w3.org/1999/02/22-rdf-syntax-ns#nil"/>
  </rdf:Description>
  <rdf:Description rdf:about="http://www.semanticweb.org/evabl45/ontologies/2023/8/untitled-ontology-86/DigitalObject">
    <rdf:type rdf:resource="http://www.w3.org/2002/07/owl#Class"/>
    <rdfs:subClassOf rdf:resource="http://w3id.org/CEON/ontology/resourceODP/Resource"/>
    <rdfs:comment>A digital object, e.g. file or other digital resource, exisiting on a computer, server, on the web etc.</rdfs:comment>
    <rdfs:label>Digital object</rdfs:label>
  </rdf:Description>
  <rdf:Description rdf:about="http://www.semanticweb.org/evabl45/ontologies/2023/8/untitled-ontology-86/DataSheet">
    <rdf:type rdf:resource="http://www.w3.org/2002/07/owl#Class"/>
    <rdfs:subClassOf rdf:resource="http://w3id.org/CEON/ontology/resourceODP/Information"/>
    <rdfs:subClassOf rdf:resource="http://www.w3.org/ns/prov#Entity"/>
    <rdfs:subClassOf rdf:nodeID="nfc0bec8256f84fce82d7a0bf9e82b550b4"/>
    <rdfs:comment>A data sheet is a collection of data about something, e.g. a set of facts about a product.</rdfs:comment>
    <rdfs:label>Data Sheet</rdfs:label>
  </rdf:Description>
  <rdf:Description rdf:nodeID="nfc0bec8256f84fce82d7a0bf9e82b550b2">
    <rdf:first rdf:resource="http://www.semanticweb.org/evabl45/ontologies/2023/8/untitled-ontology-86/DigitalObject"/>
    <rdf:rest rdf:nodeID="nfc0bec8256f84fce82d7a0bf9e82b550b3"/>
  </rdf:Description>
</rdf:RDF>
