@prefix : <http://w3id.org/CEON/ontology/quantity/> .
@prefix owl: <http://www.w3.org/2002/07/owl#> .
@prefix rdf: <http://www.w3.org/1999/02/22-rdf-syntax-ns#> .
@prefix xml: <http://www.w3.org/XML/1998/namespace> .
@prefix xsd: <http://www.w3.org/2001/XMLSchema#> .
@prefix qudt: <http://qudt.org/schema/qudt/> .
@prefix rdfs: <http://www.w3.org/2000/01/rdf-schema#> .
@prefix vann: <http://purl.org/vocab/vann/> .
@prefix dcterms: <http://purl.org/dc/terms/> .
@prefix qudt-unit: <http://qudt.org/vocab/unit/> .
@base <http://w3id.org/CEON/ontology/quantity/> .

<http://w3id.org/CEON/ontology/quantity/> rdf:type owl:Ontology ;
                                           owl:versionIRI <http://w3id.org/CEON/ontology/quantity/0.2/> ;
                                           owl:imports <http://w3id.org/CEON/ontology/qudtunit/2.1/> ;
                                           dcterms:creator "Huanyu Li" ;
                                           dcterms:contributor "Eva Blomqvist" ;
                                           dcterms:created "2024-12-31"^^xsd:date ;
                                           dcterms:issued "2025-06-30"^^xsd:date ;
                                           dcterms:publisher "Onto-DESIDE" ;
                                           dcterms:license "https://creativecommons.org/licenses/by/4.0/" ;
                                           dcterms:title "Circular Economy Ontology Network (CEON) - Quantity Module" ;
                                           vann:preferredNamespacePrefix "ceon-quantity" ;
                                           vann:preferredNamespaceUri "http://w3id.org/CEON/ontology/quantity/" ;
                                           rdfs:comment "This module defines base properties to describe quantitites with standardized units." ;
                                           rdfs:seeAlso "https://github.com/LiUSemWeb/CEON" ;
                                           owl:priorVersion 0.1 ;
                                           owl:versionInfo 0.2 .

#################################################################
#    Annotation properties
#################################################################

###  http://purl.org/dc/terms/creator
#dcterms:creator rdf:type owl:AnnotationProperty .



#################################################################
#    Object Properties
#################################################################

###  http://w3id.org/CEON/ontology/quantity/hasDimension
:hasDimension rdf:type owl:ObjectProperty ;
              rdfs:subPropertyOf qudt:quantityValue ;
              rdfs:comment "hasDimension is used to describe a dimension of a product or product object." ;
              rdfs:label "has dimension" .


###  http://w3id.org/CEON/ontology/quantity/hasDismantlingCost
:hasDismantlingCost rdf:type owl:ObjectProperty ;
                    rdfs:subPropertyOf :hasProcessCost ;
                    rdfs:comment "The cost of dismantling, expressed as an amount of money with a currency unit." ;
                    rdfs:label "has dismantling cost" .


###  http://w3id.org/CEON/ontology/quantity/hasHeight
:hasHeight rdf:type owl:ObjectProperty ;
           rdfs:subPropertyOf :hasDimension ;
           rdfs:comment "hasHeight is used to describe the height of a product or product object." ;
           rdfs:label "has height" .


###  http://w3id.org/CEON/ontology/quantity/hasLength
:hasLength rdf:type owl:ObjectProperty ;
           rdfs:subPropertyOf :hasDimension ;
           rdfs:comment "hasLength is used to describe the length of a product or product object." ;
           rdfs:label "has length" .


###  http://w3id.org/CEON/ontology/quantity/hasMarketValue
:hasMarketValue rdf:type owl:ObjectProperty ;
                rdfs:subPropertyOf qudt:quantityValue ;
                rdfs:comment "The market value, expressed as an amount of money with a currency unit." ;
                rdfs:label "has market value" .


###  http://w3id.org/CEON/ontology/quantity/hasMaximalValueIncludedOfInterval
:hasMaximalValueIncludedOfInterval rdf:type owl:ObjectProperty ;
                                   rdfs:subPropertyOf qudt:quantityValue ;
                                   rdfs:domain :QuantityInterval ;
                                   rdfs:range qudt:QuantityValue ;
                                   rdfs:comment "represents the maximum value (included) of an interval" ;
                                   rdfs:label "has maximal value included of interval" .


###  http://w3id.org/CEON/ontology/quantity/hasMaximalValueNotIncludedOfInterval
:hasMaximalValueNotIncludedOfInterval rdf:type owl:ObjectProperty ;
                                      rdfs:subPropertyOf qudt:quantityValue ;
                                      rdfs:domain :QuantityInterval ;
                                      rdfs:range qudt:QuantityValue ;
                                      rdfs:comment "represents the maximum value (not included) of an interval" ;
                                      rdfs:label "has maximal value not included of interval" .


###  http://w3id.org/CEON/ontology/quantity/hasMinimalValueIncludedOfInterval
:hasMinimalValueIncludedOfInterval rdf:type owl:ObjectProperty ;
                                   rdfs:subPropertyOf qudt:quantityValue ;
                                   rdfs:domain :QuantityInterval ;
                                   rdfs:range qudt:QuantityValue ;
                                   rdfs:comment "represents the minimal value (included) of an interval" ;
                                   rdfs:label "has minimal value included of interval" .


###  http://w3id.org/CEON/ontology/quantity/hasMinimalValueNotIncludedOfInterval
:hasMinimalValueNotIncludedOfInterval rdf:type owl:ObjectProperty ;
                                      rdfs:subPropertyOf qudt:quantityValue ;
                                      rdfs:domain :QuantityInterval ;
                                      rdfs:range qudt:QuantityValue ;
                                      rdfs:comment "represents the minimal value (not included) of an interval" ;
                                      rdfs:label "has minimal value not included of interval" .


###  http://w3id.org/CEON/ontology/quantity/hasPrice
:hasPrice rdf:type owl:ObjectProperty ;
          rdfs:subPropertyOf qudt:quantityValue ;
          rdfs:comment "represents that sth has a specific cost" ;
          rdfs:label "has price" .


###  http://w3id.org/CEON/ontology/quantity/hasProcessCost
:hasProcessCost rdf:type owl:ObjectProperty ;
                rdfs:subPropertyOf qudt:quantityValue ;
                rdfs:comment "represents that a process can have a cost" ;
                rdfs:label "has process cost" .


###  http://w3id.org/CEON/ontology/quantity/hasRecyclingCost
:hasRecyclingCost rdf:type owl:ObjectProperty ;
                  rdfs:subPropertyOf :hasProcessCost ;
                  rdfs:comment "The cost of recycling, expressed as an amount of money with a currency unit." ;
                  rdfs:label "has recycling cost" .


###  http://w3id.org/CEON/ontology/quantity/hasRefurbishmentCost
:hasRefurbishmentCost rdf:type owl:ObjectProperty ;
                      rdfs:subPropertyOf :hasProcessCost ;
                      rdfs:comment "The cost of refurbishment, expressed as an amount of money with a currency unit." ;
                      rdfs:label "has refurbishment cost" .


###  http://w3id.org/CEON/ontology/quantity/hasTestingCost
:hasTestingCost rdf:type owl:ObjectProperty ;
                rdfs:subPropertyOf :hasProcessCost ;
                rdfs:comment "The cost of testing, expressed as an amount of money with a currency unit." ;
                rdfs:label "has testing cost" .


###  http://w3id.org/CEON/ontology/quantity/hasThickness
:hasThickness rdf:type owl:ObjectProperty ;
              rdfs:subPropertyOf :hasDimension ;
              rdfs:comment "hasThickness is used to describe the thickness of a product or product object." ;
              rdfs:label "has thickness" .


###  http://w3id.org/CEON/ontology/quantity/hasTransportCost
:hasTransportCost rdf:type owl:ObjectProperty ;
                  rdfs:subPropertyOf :hasProcessCost ;
                  rdfs:comment "The cost of transportation, expressed as an amount of money with a currency unit." ;
                  rdfs:label "has transport cost" .


###  http://w3id.org/CEON/ontology/quantity/hasVolume
:hasVolume rdf:type owl:ObjectProperty ;
           rdfs:subPropertyOf qudt:quantityValue ;
           rdfs:comment "represents the volume of an object" ;
           rdfs:label "has volume" .


###  http://w3id.org/CEON/ontology/quantity/hasWeight
:hasWeight rdf:type owl:ObjectProperty ;
           rdfs:subPropertyOf qudt:quantityValue ;
           rdfs:comment "represents the weight of an object" ;
           rdfs:label "has weight" .


###  http://w3id.org/CEON/ontology/quantity/hasWidth
:hasWidth rdf:type owl:ObjectProperty ;
          rdfs:subPropertyOf :hasDimension ;
          rdfs:comment "hasWidth is used to describe the width of a product or product object." ;
          rdfs:label "has width" .


###  http://w3id.org/CEON/ontology/quantity/objectValue
:objectValue rdf:type owl:ObjectProperty ;
             rdfs:subPropertyOf qudt:hasQuantityKind ;
             rdfs:comment "objectValue is analogous to qudt:numericalValue" ;
             rdfs:label "object value" .


#################################################################
#    Data properties
#################################################################

###  http://w3id.org/CEON/ontology/quantity/numericalMaxValue
:numericalMaxValue rdf:type owl:DatatypeProperty ;
                   rdfs:range xsd:double ;
                   rdfs:comment "represents the maximal value of a quantity" ;
                   rdfs:label "numerical max value" .


###  http://w3id.org/CEON/ontology/quantity/numericalMinValue
:numericalMinValue rdf:type owl:DatatypeProperty ;
                   rdfs:subPropertyOf owl:topDataProperty ;
                   rdfs:range xsd:double ;
                   rdfs:comment "represents the minimal value of a quantity" ;
                   rdfs:label "numerical min value" .


#################################################################
#    Classes
#################################################################

###  http://w3id.org/CEON/ontology/quantity/QuantityInterval
:QuantityInterval rdf:type owl:Class ;
                  rdfs:comment "Quantity interval is an interval with two quantity values." ;
                  rdfs:label "Quantity Interval" .


#################################################################
#    Individuals
#################################################################

###  http://qudt.org/vocab/unit/EURO-PER-KiloM
qudt-unit:EURO-PER-KiloM rdf:type owl:NamedIndividual ,
                                  qudt:Unit ;
                         dcterms:description "Euro Per Kilometer (€/km) is a unit used to represent the cost or value associated with transporting a resource."^^rdf:HTML ;
                         qudt:symbol "€/km" ;
                         rdfs:label "Euro Per Kilometer" .


###  http://qudt.org/vocab/unit/EURO-PER-M2
qudt-unit:EURO-PER-M2 rdf:type owl:NamedIndividual ,
                               qudt:Unit ;
                      dcterms:description "Euro Per Square Meter (€/km) is a unit used to represent the cost or value of resource per square meter."^^rdf:HTML ;
                      qudt:symbol "€/m²" ;
                      rdfs:label "Euro Per Square Meter" .


###  http://w3id.org/CEON/ontology/quantity/Cost
:Cost rdf:type owl:NamedIndividual .


###  http://w3id.org/CEON/ontology/quantity/FloorPanel1
:FloorPanel1 rdf:type owl:NamedIndividual .


###  http://w3id.org/CEON/ontology/quantity/HIGH_QUALITY
:HIGH_QUALITY rdf:type owl:NamedIndividual .


###  http://w3id.org/CEON/ontology/quantity/LOW_QUALITY
:LOW_QUALITY rdf:type owl:NamedIndividual .


###  http://w3id.org/CEON/ontology/quantity/MEDIUM_QUALITY
:MEDIUM_QUALITY rdf:type owl:NamedIndividual .


###  http://w3id.org/CEON/ontology/quantity/Value
:Value rdf:type owl:NamedIndividual .


###  Generated by the OWL API (version 4.5.29.2024-05-13T12:11:03Z) https://github.com/owlcs/owlapi
