@prefix : <http://www.semanticweb.org/evabl45/ontologies/2023/8/untitled-ontology-86/> .
@prefix owl: <http://www.w3.org/2002/07/owl#> .
@prefix rdf: <http://www.w3.org/1999/02/22-rdf-syntax-ns#> .
@prefix xml: <http://www.w3.org/XML/1998/namespace> .
@prefix xsd: <http://www.w3.org/2001/XMLSchema#> .
@prefix rdfs: <http://www.w3.org/2000/01/rdf-schema#> .
@base <http://www.semanticweb.org/evabl45/ontologies/2023/8/untitled-ontology-86/> .

<http://w3id.org/CEON/ontology/datasheet/> rdf:type owl:Ontology ;
                                            owl:versionIRI <http://w3id.org/CEON/ontology/datasheet/0.1/> ;
                                            owl:imports <http://w3id.org/CEON/ontology/resourceODP/0.2/> ,
                                                        <http://www.w3.org/ns/prov-o-20130430> .

#################################################################
#    Object Properties
#################################################################

###  http://w3id.org/CEON/ontology/datasheet/isRealizationOf
:isRealizationOf rdf:type owl:ObjectProperty ;
                 rdfs:domain [ rdf:type owl:Class ;
                               owl:unionOf ( :DigitalObject
                                             <http://w3id.org/CEON/ontology/resourceODP/PhysicalObject>
                                           )
                             ] ;
                 rdfs:range <http://w3id.org/CEON/ontology/resourceODP/Information> ;
                 rdfs:comment "The physical or digital realisation of a piece of information, e.g. a pdf file that stores the information about a product." ;
                 rdfs:label "is realization of" .


#################################################################
#    Classes
#################################################################

###  http://w3id.org/CEON/ontology/datasheet/DataSheet
:DataSheet rdf:type owl:Class ;
           rdfs:subClassOf <http://w3id.org/CEON/ontology/resourceODP/Information> ,
                           <http://www.w3.org/ns/prov#Entity> ,
                           [ rdf:type owl:Restriction ;
                             owl:onProperty <http://w3id.org/CEON/ontology/resourceODP/containsInformation> ;
                             owl:someValuesFrom :Statement
                           ] ;
           rdfs:comment "A data sheet is a collection of data about something, e.g. a set of facts about a product." ;
           rdfs:label "Data Sheet" .


###  http://w3id.org/CEON/ontology/datasheet/DigitalObject
:DigitalObject rdf:type owl:Class ;
               rdfs:subClassOf <http://w3id.org/CEON/ontology/resourceODP/Resource> ;
               rdfs:comment "A digital object, e.g. file or other digital resource, exisiting on a computer, server, on the web etc." ;
               rdfs:label "Digital object" .


###  http://w3id.org/CEON/ontology/datasheet/Statement
:Statement rdf:type owl:Class ;
           rdfs:subClassOf <http://w3id.org/CEON/ontology/resourceODP/Information> ;
           rdfs:comment "A single fact, or statement about something. Usually contained within some larger piece of information, e.g. a document." ;
           rdfs:label "Statement" .


###  Generated by the OWL API (version 4.5.25.2023-02-15T19:15:49Z) https://github.com/owlcs/owlapi
