@prefix : <http://w3id.org/CEON/ontology/processODP/> .
@prefix dcterms: <http://purl.org/dc/terms/> .
@prefix odp: <http://www.ontologydesignpatterns.org/schemas/cpannotationschema.owl#> .
@prefix owl: <http://www.w3.org/2002/07/owl#> .
@prefix rdfs: <http://www.w3.org/2000/01/rdf-schema#> .
@prefix vann: <http://purl.org/vocab/vann/> .
@prefix xsd: <http://www.w3.org/2001/XMLSchema#> .

: a owl:Ontology ;
    dcterms:contributor "Eva Blomqvist",
        "Mikael Lindecrantz",
        "Robin Keskisärkkä" ;
    dcterms:created "2025-05-20"^^xsd:date ;
    dcterms:creator "Huanyu Li" ;
    dcterms:description "A core ODP of the CEON ontology network, defining aspects of the process concept." ;
    dcterms:issued "2025-06-30"^^xsd:date ;
    dcterms:license "https://creativecommons.org/licenses/by/4.0/" ;
    dcterms:publisher "Onto-DESIDE" ;
    dcterms:title "Circular Economy Ontology Network (CEON) - Process ODP" ;
    vann:preferredNamespacePrefix "ceon-processODP" ;
    vann:preferredNamespaceUri "http://w3id.org/CEON/ontology/processODP/" ;
    odp:coversRequirements "Covers the following requirements from Onto-DESIDE D3.1: CVN-Process-3,4,5, C3-1, C4-2, C4-5, C4-7, C4-9, C13-2, E2-6",
        "Covers the following requirements from Onto-DESIDE D3.2: CE1-1, CE3-5, CE7-4, CE7-5, CE8-2, CE10-7, CE12-1, C3-1, C4-2, C4-5, C4-7, C4-9, C13-2, E2-6" ;
    rdfs:comment "A core ODP of the CEON ontology network, defining aspects of the process concept." ;
    rdfs:seeAlso <https://github.com/LiUSemWeb/CEON> ;
    owl:priorVersion 0.4 ;
    owl:versionIRI <http://w3id.org/CEON/ontology/processODP/0.5/> ;
    owl:versionInfo 0.5 .

:Event a owl:Class ;
    rdfs:label "Event" ;
    rdfs:comment "Activities that take place within a given context or timeframe." .

:duringTime a owl:ObjectProperty ;
    rdfs:label "during time" ;
    rdfs:comment "The time interval during which a transition takes place." ;
    rdfs:range :TimeInterval ;
    rdfs:subPropertyOf :isSettingFor .

:endTime a owl:DatatypeProperty ;
    rdfs:label "end time" ;
    rdfs:comment "Represents the end time of a time interval." ;
    rdfs:domain :TimeInterval ;
    rdfs:range xsd:dateTime .

:hasInput a owl:ObjectProperty ;
    rdfs:label "has input" ;
    rdfs:comment "The inputs to this process event." ;
    rdfs:domain :Process .

:hasOutput a owl:ObjectProperty ;
    rdfs:label "has output" ;
    rdfs:comment "The output to this process event." ;
    rdfs:domain :Process .

:hasPart a owl:ObjectProperty,
        owl:TransitiveProperty ;
    rdfs:label "has part" ;
    rdfs:comment "A plan or execution can consists of several parts, which are sub-plans (or execution steps)." .

:occursAtLocation a owl:ObjectProperty ;
    rdfs:label "occurs at location" ;
    rdfs:comment "The location in which something (e.g. an execution/transition) takes place, e.g. the factory location where something is manufactured." ;
    rdfs:range <http://w3id.org/CEON/ontology/location/Location> ;
    rdfs:subPropertyOf :isSettingFor .

:startTime a owl:DatatypeProperty ;
    rdfs:label "start time" ;
    rdfs:comment "Represents the start time of a time interval." ;
    rdfs:domain :TimeInterval ;
    rdfs:range xsd:dateTime .

<http://w3id.org/CEON/ontology/location/Location> a owl:Class .

:Situation a owl:Class ;
    rdfs:label "Situation" ;
    rdfs:comment "A situation that may involve some resources and actors, i.e. a state of affairs at a certain point in time." ;
    rdfs:subClassOf [ a owl:Restriction ;
            owl:onProperty :isSettingFor ;
            owl:someValuesFrom owl:Thing ] .

:Process a owl:Class ;
    rdfs:label "Process" ;
    rdfs:comment "Set of interrelated or interacting activities that transforms inputs into outputs."@en ;
    rdfs:isDefinedBy "ISO 59004:2024  - 3.5.5 process" ;
    rdfs:seeAlso "https://ref.gs1.org/epcis/EPCISEvent" .

:TimeInterval a owl:Class ;
    rdfs:label "Time Interval" ;
    rdfs:comment "A temporal entity has a starting time and an ending time." .

:isSettingFor a owl:ObjectProperty ;
    rdfs:label "is the setting for" ;
    rdfs:comment "The thing(s) that this situation is the setting for, e.g. a resource that is in a certain state." ;
    rdfs:domain :Situation .

