<?xml version="1.0" encoding="utf-8"?>
<rdf:RDF
   xmlns:dcterms="http://purl.org/dc/terms/"
   xmlns:odp="http://www.ontologydesignpatterns.org/schemas/cpannotationschema.owl#"
   xmlns:owl="http://www.w3.org/2002/07/owl#"
   xmlns:rdf="http://www.w3.org/1999/02/22-rdf-syntax-ns#"
   xmlns:rdfs="http://www.w3.org/2000/01/rdf-schema#"
   xmlns:vann="http://purl.org/vocab/vann/"
>
  <rdf:Description rdf:about="http://w3id.org/CEON/ontology/product/Item">
    <rdf:type rdf:resource="http://www.w3.org/2002/07/owl#Class"/>
    <rdfs:subClassOf rdf:resource="http://w3id.org/CEON/ontology/resourceODP/PhysicalObject"/>
    <rdfs:subClassOf rdf:nodeID="ne6c0ad3282a0432d8ac896e6816386d7b22"/>
    <rdfs:comment xml:lang="en">An item is a physical object put into a market for sale, i.e. corresponding to an individual of a product. The item can be a thing that grows naturally or produced through some chemical or manufacturing processes.</rdfs:comment>
    <rdfs:label xml:lang="en">Item</rdfs:label>
  </rdf:Description>
  <rdf:Description rdf:nodeID="ne6c0ad3282a0432d8ac896e6816386d7b22">
    <rdf:type rdf:resource="http://www.w3.org/2002/07/owl#Restriction"/>
    <owl:onProperty rdf:resource="http://w3id.org/CEON/ontology/product/modelledBy"/>
    <owl:qualifiedCardinality rdf:datatype="http://www.w3.org/2001/XMLSchema#nonNegativeInteger">1</owl:qualifiedCardinality>
    <owl:onClass rdf:resource="http://w3id.org/CEON/ontology/product/Product"/>
  </rdf:Description>
  <rdf:Description rdf:about="http://w3id.org/CEON/ontology/product/locationOfAssembly">
    <rdf:type rdf:resource="http://www.w3.org/2002/07/owl#DatatypeProperty"/>
    <rdfs:domain rdf:nodeID="ne6c0ad3282a0432d8ac896e6816386d7b13"/>
    <rdfs:range rdf:resource="http://www.w3.org/2001/XMLSchema#string"/>
    <rdfs:comment>Used to represent the location of assembly of a product or product object</rdfs:comment>
    <rdfs:label>Location of assembly</rdfs:label>
  </rdf:Description>
  <rdf:Description rdf:nodeID="ne6c0ad3282a0432d8ac896e6816386d7b20">
    <rdf:first rdf:resource="http://w3id.org/CEON/ontology/product/Item"/>
    <rdf:rest rdf:nodeID="ne6c0ad3282a0432d8ac896e6816386d7b21"/>
  </rdf:Description>
  <rdf:Description rdf:about="http://w3id.org/CEON/ontology/product/countryOfManufacture">
    <rdf:type rdf:resource="http://www.w3.org/2002/07/owl#DatatypeProperty"/>
    <rdfs:subPropertyOf rdf:resource="http://w3id.org/CEON/ontology/product/locationOfManufacture"/>
    <rdfs:comment>Used to represent the country of manufacture of a product or product object</rdfs:comment>
    <rdfs:label>Country of manufacture</rdfs:label>
  </rdf:Description>
  <rdf:Description rdf:about="http://w3id.org/CEON/ontology/product/locationOfOrigin">
    <rdf:type rdf:resource="http://www.w3.org/2002/07/owl#DatatypeProperty"/>
    <rdfs:domain rdf:nodeID="ne6c0ad3282a0432d8ac896e6816386d7b19"/>
    <rdfs:range rdf:resource="http://www.w3.org/2001/XMLSchema#string"/>
    <rdfs:comment>Used to represent the location of origin of a product or product object</rdfs:comment>
    <rdfs:label>Location of origin</rdfs:label>
  </rdf:Description>
  <rdf:Description rdf:about="http://w3id.org/CEON/ontology/resourceODP/PhysicalObject">
    <rdf:type rdf:resource="http://www.w3.org/2002/07/owl#Class"/>
  </rdf:Description>
  <rdf:Description rdf:about="http://w3id.org/CEON/ontology/product/associatedWithProductModel">
    <rdf:type rdf:resource="http://www.w3.org/2002/07/owl#ObjectProperty"/>
    <rdfs:domain rdf:resource="http://w3id.org/CEON/ontology/product/ProductComposition"/>
    <rdfs:range rdf:resource="http://w3id.org/CEON/ontology/product/Product"/>
    <rdfs:comment xml:lang="en">associatedWithProductModel intends to represent the product model to which a product compopsition information regards to.</rdfs:comment>
    <rdfs:label xml:lang="en">associated with product model</rdfs:label>
  </rdf:Description>
  <rdf:Description rdf:about="http://w3id.org/CEON/ontology/product/hasCertificate">
    <rdf:type rdf:resource="http://www.w3.org/2002/07/owl#DatatypeProperty"/>
    <rdfs:domain rdf:resource="http://w3id.org/CEON/ontology/product/Compliance"/>
    <rdfs:comment>Link to the the certificate that certifies the compliance</rdfs:comment>
    <rdfs:label>has certificate</rdfs:label>
  </rdf:Description>
  <rdf:Description rdf:about="http://w3id.org/CEON/ontology/product/hasProductComponent">
    <rdf:type rdf:resource="http://www.w3.org/2002/07/owl#ObjectProperty"/>
    <rdfs:domain rdf:resource="http://w3id.org/CEON/ontology/product/Product"/>
    <rdfs:range rdf:resource="http://w3id.org/CEON/ontology/product/Product"/>
    <rdfs:comment xml:lang="en">hasProductComponent intends to represent that a product can have other product components.</rdfs:comment>
    <rdfs:label xml:lang="en">has product component</rdfs:label>
  </rdf:Description>
  <rdf:Description rdf:about="http://w3id.org/CEON/ontology/product/hasCompliance">
    <rdf:type rdf:resource="http://www.w3.org/2002/07/owl#ObjectProperty"/>
    <rdfs:domain rdf:nodeID="ne6c0ad3282a0432d8ac896e6816386d7b5"/>
    <rdfs:range rdf:resource="http://w3id.org/CEON/ontology/product/Compliance"/>
    <rdfs:comment>Used to link something (e.g., product or process) to a compliance.</rdfs:comment>
    <rdfs:label>has compliance</rdfs:label>
  </rdf:Description>
  <rdf:Description rdf:about="http://w3id.org/CEON/ontology/product/countryOfOrigin">
    <rdf:type rdf:resource="http://www.w3.org/2002/07/owl#DatatypeProperty"/>
    <rdfs:subPropertyOf rdf:resource="http://w3id.org/CEON/ontology/product/locationOfOrigin"/>
    <rdfs:comment>Used to represent the country of origin of a product or product object</rdfs:comment>
    <rdfs:label>Country of origin</rdfs:label>
  </rdf:Description>
  <rdf:Description rdf:nodeID="ne6c0ad3282a0432d8ac896e6816386d7b24">
    <rdf:type rdf:resource="http://www.w3.org/2002/07/owl#Restriction"/>
    <owl:onProperty rdf:resource="http://w3id.org/CEON/ontology/product/hasComposition"/>
    <owl:someValuesFrom rdf:resource="http://w3id.org/CEON/ontology/product/MatterComposition"/>
  </rdf:Description>
  <rdf:Description rdf:nodeID="ne6c0ad3282a0432d8ac896e6816386d7b12">
    <rdf:first rdf:resource="http://w3id.org/CEON/ontology/resourceODP/PhysicalObject"/>
    <rdf:rest rdf:resource="http://www.w3.org/1999/02/22-rdf-syntax-ns#nil"/>
  </rdf:Description>
  <rdf:Description rdf:about="http://w3id.org/CEON/ontology/product/hasComposition">
    <rdf:type rdf:resource="http://www.w3.org/2002/07/owl#ObjectProperty"/>
    <rdfs:domain rdf:nodeID="ne6c0ad3282a0432d8ac896e6816386d7b10"/>
    <rdfs:range rdf:resource="http://w3id.org/CEON/ontology/resourceODP/Composition"/>
    <rdfs:comment xml:lang="en">hasComposition intends to represent that a product model or physical object can have compostition information.</rdfs:comment>
    <rdfs:label>has composition</rdfs:label>
  </rdf:Description>
  <rdf:Description rdf:about="http://w3id.org/CEON/ontology/product/">
    <rdf:type rdf:resource="http://www.w3.org/2002/07/owl#Ontology"/>
    <owl:versionIRI rdf:resource="http://w3id.org/CEON/ontology/product/0.4/"/>
    <owl:imports rdf:resource="http://w3id.org/CEON/ontology/actorODP/0.3/"/>
    <owl:imports rdf:resource="http://w3id.org/CEON/ontology/resourceODP/0.3/"/>
    <dcterms:contributor>Eva Blomqvist</dcterms:contributor>
    <dcterms:contributor>Mikael Lindecrantz</dcterms:contributor>
    <dcterms:contributor>Robin Keskisärkkä</dcterms:contributor>
    <dcterms:created>2023-03-16</dcterms:created>
    <dcterms:creator>Huanyu Li</dcterms:creator>
    <dcterms:description>The Product module of CEON (Circular Economy Ontology Network).</dcterms:description>
    <dcterms:license>https://creativecommons.org/licenses/by/4.0/</dcterms:license>
    <dcterms:title>Circular Economy Ontology Network (CEON) - Product Module</dcterms:title>
    <vann:preferredNamespacePrefix>product</vann:preferredNamespacePrefix>
    <vann:preferredNamespaceUri>http://w3id.org/CEON/ontology/product/</vann:preferredNamespaceUri>
    <odp:coversRequirements>In addition to requirements covered by imported ODPs, covers the following requirements from Onto-DESIDE D3.1: CVN-Resource-2, CVN-ResrouceType-4, C11-2, C12-1, C13-3, E2-1, T8-3.</odp:coversRequirements>
    <odp:coversRequirements>In addition to requirements covered by imported ODPs, covers the following requirements from Onto-DESIDE D2.3: CE5-2, C11-2, C12-1, C13-3, E2-1, T8-3.</odp:coversRequirements>
    <rdfs:seeAlso rdf:resource="https://github.com/LiUSemWeb/CEON"/>
    <owl:versionInfo rdf:datatype="http://www.w3.org/2001/XMLSchema#decimal">0.4</owl:versionInfo>
  </rdf:Description>
  <rdf:Description rdf:nodeID="ne6c0ad3282a0432d8ac896e6816386d7b15">
    <rdf:first rdf:resource="http://w3id.org/CEON/ontology/product/Product"/>
    <rdf:rest rdf:resource="http://www.w3.org/1999/02/22-rdf-syntax-ns#nil"/>
  </rdf:Description>
  <rdf:Description rdf:nodeID="ne6c0ad3282a0432d8ac896e6816386d7b5">
    <rdf:type rdf:resource="http://www.w3.org/2002/07/owl#Class"/>
    <owl:unionOf rdf:nodeID="ne6c0ad3282a0432d8ac896e6816386d7b6"/>
  </rdf:Description>
  <rdf:Description rdf:about="http://purl.org/dc/terms/description">
    <rdf:type rdf:resource="http://www.w3.org/2002/07/owl#AnnotationProperty"/>
  </rdf:Description>
  <rdf:Description rdf:about="http://w3id.org/CEON/ontology/product/locationOfManufacture">
    <rdf:type rdf:resource="http://www.w3.org/2002/07/owl#DatatypeProperty"/>
    <rdfs:domain rdf:nodeID="ne6c0ad3282a0432d8ac896e6816386d7b16"/>
    <rdfs:range rdf:resource="http://www.w3.org/2001/XMLSchema#string"/>
    <rdfs:comment>Used to represent the location of manufacture of a product or product object</rdfs:comment>
    <rdfs:label>Location of manufacture</rdfs:label>
  </rdf:Description>
  <rdf:Description rdf:nodeID="ne6c0ad3282a0432d8ac896e6816386d7b3">
    <rdf:first rdf:resource="http://w3id.org/CEON/ontology/product/Product"/>
    <rdf:rest rdf:nodeID="ne6c0ad3282a0432d8ac896e6816386d7b4"/>
  </rdf:Description>
  <rdf:Description rdf:nodeID="ne6c0ad3282a0432d8ac896e6816386d7b27">
    <rdf:type rdf:resource="http://www.w3.org/2002/07/owl#Restriction"/>
    <owl:onProperty rdf:resource="http://w3id.org/CEON/ontology/product/associatedWithProductObject"/>
    <owl:qualifiedCardinality rdf:datatype="http://www.w3.org/2001/XMLSchema#nonNegativeInteger">1</owl:qualifiedCardinality>
    <owl:onClass rdf:resource="http://w3id.org/CEON/ontology/product/Item"/>
  </rdf:Description>
  <rdf:Description rdf:nodeID="ne6c0ad3282a0432d8ac896e6816386d7b9">
    <rdf:first rdf:resource="http://w3id.org/CEON/ontology/product/Product"/>
    <rdf:rest rdf:resource="http://www.w3.org/1999/02/22-rdf-syntax-ns#nil"/>
  </rdf:Description>
  <rdf:Description rdf:about="http://w3id.org/CEON/ontology/product/Solution">
    <rdf:type rdf:resource="http://www.w3.org/2002/07/owl#Class"/>
    <rdfs:comment xml:lang="en">Product or service, or a combination thereof, that fulfils a need of an interested party.</rdfs:comment>
    <rdfs:isDefinedBy>ISO 59004:2024 - 3.2.1 solution</rdfs:isDefinedBy>
    <rdfs:label xml:lang="en">Solution</rdfs:label>
  </rdf:Description>
  <rdf:Description rdf:nodeID="ne6c0ad3282a0432d8ac896e6816386d7b23">
    <rdf:type rdf:resource="http://www.w3.org/2002/07/owl#Restriction"/>
    <owl:onProperty rdf:resource="http://w3id.org/CEON/ontology/product/associatedWithMatter"/>
    <owl:qualifiedCardinality rdf:datatype="http://www.w3.org/2001/XMLSchema#nonNegativeInteger">1</owl:qualifiedCardinality>
    <owl:onClass rdf:resource="http://w3id.org/CEON/ontology/resourceODP/Matter"/>
  </rdf:Description>
  <rdf:Description rdf:nodeID="ne6c0ad3282a0432d8ac896e6816386d7b13">
    <rdf:type rdf:resource="http://www.w3.org/2002/07/owl#Class"/>
    <owl:unionOf rdf:nodeID="ne6c0ad3282a0432d8ac896e6816386d7b14"/>
  </rdf:Description>
  <rdf:Description rdf:about="http://w3id.org/CEON/ontology/resourceODP/Composition">
    <rdf:type rdf:resource="http://www.w3.org/2002/07/owl#Class"/>
    <rdfs:subClassOf rdf:resource="http://w3id.org/CEON/ontology/actorODP/ResourceRelation"/>
  </rdf:Description>
  <rdf:Description rdf:about="http://w3id.org/CEON/ontology/product/MatterComposition">
    <rdf:type rdf:resource="http://www.w3.org/2002/07/owl#Class"/>
    <rdfs:subClassOf rdf:resource="http://w3id.org/CEON/ontology/resourceODP/Composition"/>
    <rdfs:subClassOf rdf:nodeID="ne6c0ad3282a0432d8ac896e6816386d7b23"/>
    <rdfs:comment xml:lang="en">A product composition is the composed information of a product in terms of a specific component, in which such a component is also a matter.</rdfs:comment>
    <rdfs:label xml:lang="en">Matter composition</rdfs:label>
  </rdf:Description>
  <rdf:Description rdf:about="http://w3id.org/CEON/ontology/product/Product">
    <rdf:type rdf:resource="http://www.w3.org/2002/07/owl#Class"/>
    <rdfs:subClassOf rdf:resource="http://w3id.org/CEON/ontology/product/Solution"/>
    <rdfs:subClassOf rdf:nodeID="ne6c0ad3282a0432d8ac896e6816386d7b24"/>
    <rdfs:subClassOf rdf:nodeID="ne6c0ad3282a0432d8ac896e6816386d7b25"/>
    <rdfs:comment xml:lang="en">Physical-based object designed for or utilized with a purpose. A product can be, for example: goods of any type; hardware (e.g. engine mechanical part, spare parts, consumables); electrical or electronic hardware devices or components (e.g. computers, communication equipment and sensors); processed materials (e.g. lubricant, cement).</rdfs:comment>
    <rdfs:comment xml:lang="en">Represents the common sense notion of a product, i.e. the abstract notion of a product type, which is a model that is used for manufacturing items of that product.</rdfs:comment>
    <rdfs:isDefinedBy>ISO 59004:2024 -3.2.2 product</rdfs:isDefinedBy>
    <rdfs:label xml:lang="en">Product</rdfs:label>
  </rdf:Description>
  <rdf:Description rdf:nodeID="ne6c0ad3282a0432d8ac896e6816386d7b8">
    <rdf:first rdf:resource="http://w3id.org/CEON/ontology/product/Item"/>
    <rdf:rest rdf:nodeID="ne6c0ad3282a0432d8ac896e6816386d7b9"/>
  </rdf:Description>
  <rdf:Description rdf:about="http://w3id.org/CEON/ontology/product/complianceWith">
    <rdf:type rdf:resource="http://www.w3.org/2002/07/owl#ObjectProperty"/>
    <rdfs:domain rdf:resource="http://w3id.org/CEON/ontology/product/Compliance"/>
    <rdfs:comment>Represents what the compliance is compliant with (e.g. a standard or regulation).</rdfs:comment>
    <rdfs:label>Compliance with</rdfs:label>
  </rdf:Description>
  <rdf:Description rdf:about="http://w3id.org/CEON/ontology/product/ProductComposition">
    <rdf:type rdf:resource="http://www.w3.org/2002/07/owl#Class"/>
    <rdfs:subClassOf rdf:resource="http://w3id.org/CEON/ontology/resourceODP/Composition"/>
    <rdfs:subClassOf rdf:nodeID="ne6c0ad3282a0432d8ac896e6816386d7b26"/>
    <rdfs:comment xml:lang="en">A product composition is the composed information of a product in terms of a specific component, in which such a component is also a product.</rdfs:comment>
    <rdfs:label xml:lang="en">Product composition</rdfs:label>
  </rdf:Description>
  <rdf:Description rdf:nodeID="ne6c0ad3282a0432d8ac896e6816386d7b1">
    <rdf:type rdf:resource="http://www.w3.org/2002/07/owl#Class"/>
    <owl:unionOf rdf:nodeID="ne6c0ad3282a0432d8ac896e6816386d7b2"/>
  </rdf:Description>
  <rdf:Description rdf:about="http://purl.org/dc/terms/creator">
    <rdf:type rdf:resource="http://www.w3.org/2002/07/owl#AnnotationProperty"/>
  </rdf:Description>
  <rdf:Description rdf:about="http://w3id.org/CEON/ontology/product/batchOfProduct">
    <rdf:type rdf:resource="http://www.w3.org/2002/07/owl#ObjectProperty"/>
    <rdfs:domain rdf:resource="http://w3id.org/CEON/ontology/resourceODP/BatchOfObjects"/>
    <rdfs:range rdf:resource="http://w3id.org/CEON/ontology/product/Product"/>
    <rdfs:comment xml:lang="en">batchOfProduct intends to represent what is the model product of a batch of objects.</rdfs:comment>
    <rdfs:label xml:lang="en">batch of products</rdfs:label>
  </rdf:Description>
  <rdf:Description rdf:about="http://w3id.org/CEON/ontology/product/compositionOf">
    <rdf:type rdf:resource="http://www.w3.org/2002/07/owl#ObjectProperty"/>
    <rdfs:domain rdf:resource="http://w3id.org/CEON/ontology/resourceODP/Composition"/>
    <rdfs:range rdf:nodeID="ne6c0ad3282a0432d8ac896e6816386d7b1"/>
    <rdfs:comment>Represents what the composition is a composition of (i.e., the product, the product object or matter that is broken down into its components).</rdfs:comment>
    <rdfs:label>composition of</rdfs:label>
  </rdf:Description>
  <rdf:Description rdf:about="http://purl.org/dc/terms/created">
    <rdf:type rdf:resource="http://www.w3.org/2002/07/owl#AnnotationProperty"/>
  </rdf:Description>
  <rdf:Description rdf:nodeID="ne6c0ad3282a0432d8ac896e6816386d7b17">
    <rdf:first rdf:resource="http://w3id.org/CEON/ontology/product/Item"/>
    <rdf:rest rdf:nodeID="ne6c0ad3282a0432d8ac896e6816386d7b18"/>
  </rdf:Description>
  <rdf:Description rdf:about="http://www.ontologydesignpatterns.org/schemas/cpannotationschema.owl#coversRequirements">
    <rdf:type rdf:resource="http://www.w3.org/2002/07/owl#AnnotationProperty"/>
  </rdf:Description>
  <rdf:Description rdf:about="http://w3id.org/CEON/ontology/product/modelledBy">
    <rdf:type rdf:resource="http://www.w3.org/2002/07/owl#ObjectProperty"/>
    <rdfs:domain rdf:resource="http://w3id.org/CEON/ontology/product/Item"/>
    <rdfs:range rdf:resource="http://w3id.org/CEON/ontology/product/Product"/>
    <rdfs:comment xml:lang="en">modelledBy intends to represent that product objects follow particular product models.</rdfs:comment>
    <rdfs:label xml:lang="en">modelled by</rdfs:label>
  </rdf:Description>
  <rdf:Description rdf:nodeID="ne6c0ad3282a0432d8ac896e6816386d7b14">
    <rdf:first rdf:resource="http://w3id.org/CEON/ontology/product/Item"/>
    <rdf:rest rdf:nodeID="ne6c0ad3282a0432d8ac896e6816386d7b15"/>
  </rdf:Description>
  <rdf:Description rdf:about="http://w3id.org/CEON/ontology/actorODP/Actor">
    <rdf:type rdf:resource="http://www.w3.org/2002/07/owl#Class"/>
  </rdf:Description>
  <rdf:Description rdf:nodeID="ne6c0ad3282a0432d8ac896e6816386d7b10">
    <rdf:type rdf:resource="http://www.w3.org/2002/07/owl#Class"/>
    <owl:unionOf rdf:nodeID="ne6c0ad3282a0432d8ac896e6816386d7b11"/>
  </rdf:Description>
  <rdf:Description rdf:about="http://w3id.org/CEON/ontology/product/associatedWithProductObject">
    <rdf:type rdf:resource="http://www.w3.org/2002/07/owl#ObjectProperty"/>
    <rdfs:subPropertyOf rdf:resource="http://www.w3.org/2002/07/owl#topObjectProperty"/>
    <rdfs:domain rdf:resource="http://w3id.org/CEON/ontology/product/ProductObjectComposition"/>
    <rdfs:range rdf:resource="http://w3id.org/CEON/ontology/product/Item"/>
    <rdfs:comment>associatedWithProductObject intends to represent the item (product object) to which a product object compopsition information regards to.</rdfs:comment>
    <rdfs:label>associated with product object</rdfs:label>
  </rdf:Description>
  <rdf:Description rdf:about="http://w3id.org/CEON/ontology/processODP/Process">
    <rdf:type rdf:resource="http://www.w3.org/2002/07/owl#Class"/>
  </rdf:Description>
  <rdf:Description rdf:about="http://purl.org/dc/terms/title">
    <rdf:type rdf:resource="http://www.w3.org/2002/07/owl#AnnotationProperty"/>
  </rdf:Description>
  <rdf:Description rdf:about="http://w3id.org/CEON/ontology/product/compositionQuantity">
    <rdf:type rdf:resource="http://www.w3.org/2002/07/owl#DatatypeProperty"/>
    <rdfs:domain rdf:resource="http://w3id.org/CEON/ontology/resourceODP/Composition"/>
    <rdfs:range rdf:resource="http://www.w3.org/2001/XMLSchema#double"/>
    <rdfs:comment>compositionQuantity represents the quantity of elements of a composition.</rdfs:comment>
    <rdfs:label xml:lang="en">Composition quantity</rdfs:label>
  </rdf:Description>
  <rdf:Description rdf:about="http://purl.org/vocab/vann/preferredNamespacePrefix">
    <rdf:type rdf:resource="http://www.w3.org/2002/07/owl#AnnotationProperty"/>
  </rdf:Description>
  <rdf:Description rdf:nodeID="ne6c0ad3282a0432d8ac896e6816386d7b7">
    <rdf:first rdf:resource="http://w3id.org/CEON/ontology/processODP/Process"/>
    <rdf:rest rdf:nodeID="ne6c0ad3282a0432d8ac896e6816386d7b8"/>
  </rdf:Description>
  <rdf:Description rdf:nodeID="ne6c0ad3282a0432d8ac896e6816386d7b19">
    <rdf:type rdf:resource="http://www.w3.org/2002/07/owl#Class"/>
    <owl:unionOf rdf:nodeID="ne6c0ad3282a0432d8ac896e6816386d7b20"/>
  </rdf:Description>
  <rdf:Description rdf:about="http://purl.org/vocab/vann/preferredNamespaceUri">
    <rdf:type rdf:resource="http://www.w3.org/2002/07/owl#AnnotationProperty"/>
  </rdf:Description>
  <rdf:Description rdf:nodeID="ne6c0ad3282a0432d8ac896e6816386d7b21">
    <rdf:first rdf:resource="http://w3id.org/CEON/ontology/product/Product"/>
    <rdf:rest rdf:resource="http://www.w3.org/1999/02/22-rdf-syntax-ns#nil"/>
  </rdf:Description>
  <rdf:Description rdf:nodeID="ne6c0ad3282a0432d8ac896e6816386d7b25">
    <rdf:type rdf:resource="http://www.w3.org/2002/07/owl#Restriction"/>
    <owl:onProperty rdf:resource="http://w3id.org/CEON/ontology/product/hasComposition"/>
    <owl:someValuesFrom rdf:resource="http://w3id.org/CEON/ontology/product/ProductComposition"/>
  </rdf:Description>
  <rdf:Description rdf:nodeID="ne6c0ad3282a0432d8ac896e6816386d7b11">
    <rdf:first rdf:resource="http://w3id.org/CEON/ontology/product/Product"/>
    <rdf:rest rdf:nodeID="ne6c0ad3282a0432d8ac896e6816386d7b12"/>
  </rdf:Description>
  <rdf:Description rdf:about="http://w3id.org/CEON/ontology/product/hasProductObjectComponent">
    <rdf:type rdf:resource="http://www.w3.org/2002/07/owl#ObjectProperty"/>
    <rdfs:domain rdf:resource="http://w3id.org/CEON/ontology/product/Item"/>
    <rdfs:range rdf:resource="http://w3id.org/CEON/ontology/product/Item"/>
    <rdfs:label>has product object component</rdfs:label>
  </rdf:Description>
  <rdf:Description rdf:about="http://w3id.org/CEON/ontology/resourceODP/BatchOfObjects">
    <rdf:type rdf:resource="http://www.w3.org/2002/07/owl#Class"/>
    <rdfs:subClassOf rdf:nodeID="ne6c0ad3282a0432d8ac896e6816386d7b28"/>
  </rdf:Description>
  <rdf:Description rdf:nodeID="ne6c0ad3282a0432d8ac896e6816386d7b4">
    <rdf:first rdf:resource="http://w3id.org/CEON/ontology/resourceODP/Matter"/>
    <rdf:rest rdf:resource="http://www.w3.org/1999/02/22-rdf-syntax-ns#nil"/>
  </rdf:Description>
  <rdf:Description rdf:nodeID="ne6c0ad3282a0432d8ac896e6816386d7b16">
    <rdf:type rdf:resource="http://www.w3.org/2002/07/owl#Class"/>
    <owl:unionOf rdf:nodeID="ne6c0ad3282a0432d8ac896e6816386d7b17"/>
  </rdf:Description>
  <rdf:Description rdf:about="http://w3id.org/CEON/ontology/product/Compliance">
    <rdf:type rdf:resource="http://www.w3.org/2002/07/owl#Class"/>
    <rdfs:comment>Represents that something is compliant with some standard or has a received a certain certification.</rdfs:comment>
    <rdfs:label>Compliance</rdfs:label>
  </rdf:Description>
  <rdf:Description rdf:about="http://w3id.org/CEON/ontology/product/associatedWithMatter">
    <rdf:type rdf:resource="http://www.w3.org/2002/07/owl#ObjectProperty"/>
    <rdfs:domain rdf:resource="http://w3id.org/CEON/ontology/product/MatterComposition"/>
    <rdfs:range rdf:resource="http://w3id.org/CEON/ontology/resourceODP/Matter"/>
    <rdfs:comment xml:lang="en">associatedWithMatter intends to represent the matter to which a matter compopsition information regards to.</rdfs:comment>
    <rdfs:label xml:lang="en">associated with matter</rdfs:label>
  </rdf:Description>
  <rdf:Description rdf:nodeID="ne6c0ad3282a0432d8ac896e6816386d7b26">
    <rdf:type rdf:resource="http://www.w3.org/2002/07/owl#Restriction"/>
    <owl:onProperty rdf:resource="http://w3id.org/CEON/ontology/product/associatedWithProductModel"/>
    <owl:qualifiedCardinality rdf:datatype="http://www.w3.org/2001/XMLSchema#nonNegativeInteger">1</owl:qualifiedCardinality>
    <owl:onClass rdf:resource="http://w3id.org/CEON/ontology/product/Product"/>
  </rdf:Description>
  <rdf:Description rdf:nodeID="ne6c0ad3282a0432d8ac896e6816386d7b2">
    <rdf:first rdf:resource="http://w3id.org/CEON/ontology/product/Item"/>
    <rdf:rest rdf:nodeID="ne6c0ad3282a0432d8ac896e6816386d7b3"/>
  </rdf:Description>
  <rdf:Description rdf:about="http://w3id.org/CEON/ontology/resourceODP/Matter">
    <rdf:type rdf:resource="http://www.w3.org/2002/07/owl#Class"/>
  </rdf:Description>
  <rdf:Description rdf:nodeID="ne6c0ad3282a0432d8ac896e6816386d7b18">
    <rdf:first rdf:resource="http://w3id.org/CEON/ontology/product/Product"/>
    <rdf:rest rdf:resource="http://www.w3.org/1999/02/22-rdf-syntax-ns#nil"/>
  </rdf:Description>
  <rdf:Description rdf:about="http://w3id.org/CEON/ontology/product/countryOfAssembly">
    <rdf:type rdf:resource="http://www.w3.org/2002/07/owl#DatatypeProperty"/>
    <rdfs:subPropertyOf rdf:resource="http://w3id.org/CEON/ontology/product/locationOfAssembly"/>
    <rdfs:comment>Used to represent the country of assembly of a product or product object</rdfs:comment>
    <rdfs:label>Country of assembly</rdfs:label>
  </rdf:Description>
  <rdf:Description rdf:about="http://w3id.org/CEON/ontology/actorODP/ResourceRelation">
    <rdf:type rdf:resource="http://www.w3.org/2002/07/owl#Class"/>
  </rdf:Description>
  <rdf:Description rdf:about="http://w3id.org/CEON/ontology/product/ProductObjectComposition">
    <rdf:type rdf:resource="http://www.w3.org/2002/07/owl#Class"/>
    <rdfs:subClassOf rdf:resource="http://w3id.org/CEON/ontology/resourceODP/Composition"/>
    <rdfs:subClassOf rdf:nodeID="ne6c0ad3282a0432d8ac896e6816386d7b27"/>
    <rdfs:comment>A product object composition is the composed information of a product object in terms of a specific component, in which such a component is also a product object.</rdfs:comment>
    <rdfs:label>Product Object Composition</rdfs:label>
  </rdf:Description>
  <rdf:Description rdf:nodeID="ne6c0ad3282a0432d8ac896e6816386d7b6">
    <rdf:first rdf:resource="http://w3id.org/CEON/ontology/actorODP/Actor"/>
    <rdf:rest rdf:nodeID="ne6c0ad3282a0432d8ac896e6816386d7b7"/>
  </rdf:Description>
  <rdf:Description rdf:nodeID="ne6c0ad3282a0432d8ac896e6816386d7b28">
    <rdf:type rdf:resource="http://www.w3.org/2002/07/owl#Restriction"/>
    <owl:onProperty rdf:resource="http://w3id.org/CEON/ontology/product/batchOfProduct"/>
    <owl:qualifiedCardinality rdf:datatype="http://www.w3.org/2001/XMLSchema#nonNegativeInteger">1</owl:qualifiedCardinality>
    <owl:onClass rdf:resource="http://w3id.org/CEON/ontology/product/Product"/>
  </rdf:Description>
  <rdf:Description rdf:about="http://purl.org/dc/terms/contributor">
    <rdf:type rdf:resource="http://www.w3.org/2002/07/owl#AnnotationProperty"/>
  </rdf:Description>
  <rdf:Description rdf:about="http://purl.org/dc/terms/license">
    <rdf:type rdf:resource="http://www.w3.org/2002/07/owl#AnnotationProperty"/>
  </rdf:Description>
</rdf:RDF>
