<?xml version="1.0" encoding="utf-8"?>
<rdf:RDF
   xmlns:dcterms="http://purl.org/dc/terms/"
   xmlns:owl="http://www.w3.org/2002/07/owl#"
   xmlns:rdf="http://www.w3.org/1999/02/22-rdf-syntax-ns#"
   xmlns:rdfs="http://www.w3.org/2000/01/rdf-schema#"
   xmlns:vann="http://purl.org/vocab/vann/"
>
  <rdf:Description rdf:about="http://w3id.org/CEON/ontology/provenance/Statement">
    <rdf:type rdf:resource="http://www.w3.org/2002/07/owl#Class"/>
    <rdfs:subClassOf rdf:resource="http://www.w3.org/ns/prov#Entity"/>
    <rdfs:comment>Generic class representing the concept of a statement, i.e. some piece of information, fact etc that is expressed in the data. Effectively used to reify relations (triples) in the data, and express information about them.</rdfs:comment>
    <rdfs:label>statement</rdfs:label>
  </rdf:Description>
  <rdf:Description rdf:about="http://w3id.org/CEON/ontology/provenance/">
    <rdf:type rdf:resource="http://www.w3.org/2002/07/owl#Ontology"/>
    <owl:versionIRI rdf:resource="http://w3id.org/CEON/ontology/provenance/0.1/"/>
    <owl:imports rdf:resource="http://w3id.org/CEON/ontology/resourceODP/0.2/"/>
    <owl:imports rdf:resource="http://www.w3.org/ns/prov-o-20130430"/>
    <dcterms:contributor>Huanyu Li</dcterms:contributor>
    <dcterms:contributor>Mikael Lindecrantz</dcterms:contributor>
    <dcterms:contributor>Robin Keskisärkkä</dcterms:contributor>
    <dcterms:created>2023-09-18</dcterms:created>
    <dcterms:creator>Eva Blomqvist</dcterms:creator>
    <dcterms:description>A specialisation of PROV-O for expressing provenance of CEON resources.</dcterms:description>
    <dcterms:license>https://github.com/LiUSemWeb/CEON/blob/master/LICENSE</dcterms:license>
    <dcterms:title>Circular Economy Ontology Network (CEON) - Provenance</dcterms:title>
    <vann:preferredNamespacePrefix>CEONprov</vann:preferredNamespacePrefix>
    <vann:preferredNamespaceUri>http://w3id.org/CEON/ontology/provenance/</vann:preferredNamespaceUri>
    <owl:versionInfo>0.1</owl:versionInfo>
  </rdf:Description>
  <rdf:Description rdf:about="http://w3id.org/CEON/ontology/provenance/statementValue">
    <rdf:type rdf:resource="http://www.w3.org/2002/07/owl#DatatypeProperty"/>
    <rdfs:domain rdf:resource="http://w3id.org/CEON/ontology/provenance/Statement"/>
    <rdfs:comment>Generic property to express values, e.g. literals, that are involved in this statement.</rdfs:comment>
    <rdfs:label>statement value</rdfs:label>
  </rdf:Description>
  <rdf:Description rdf:about="http://w3id.org/CEON/ontology/provenance/statementAbout">
    <rdf:type rdf:resource="http://www.w3.org/2002/07/owl#ObjectProperty"/>
    <rdfs:domain rdf:resource="http://w3id.org/CEON/ontology/provenance/Statement"/>
    <rdfs:comment>Generic property to express what the statement is about, i.e. what is involved in the statement.</rdfs:comment>
    <rdfs:label>statement about</rdfs:label>
  </rdf:Description>
  <rdf:Description rdf:about="http://w3id.org/CEON/ontology/resourceODP/Resource">
    <rdfs:subClassOf rdf:resource="http://www.w3.org/ns/prov#Entity"/>
  </rdf:Description>
</rdf:RDF>
